mem safety for Poly1305 + refactoring and various fixes

lib/hst/ml/Hacl_UInt64.mli
@@ -56,11 +56,11 @@ val op_Hat_Hat:uint64 -> uint64 -> uint64
 val op_Hat_Star_Hat: uint64 -> uint64 -> uint128
                   
 val op_Plus_Hat: uint64 -> uint64 -> uint64
-val op_Plus_Hat_Percent: uint64 -> uint64 -> uint64
+val op_Plus_Percent_Hat: uint64 -> uint64 -> uint64
 val op_Subtraction_Hat: uint64 -> uint64 -> uint64
-val op_Subtraction_Hat_Percent: uint64 -> uint64 -> uint64
+val op_Subtraction_Percent_Hat: uint64 -> uint64 -> uint64
 val op_Star_Hat: uint64 -> uint64 -> uint64
-val op_Star_Hat_Percent: uint64 -> uint64 -> uint64
+val op_Star_Percent_Hat: uint64 -> uint64 -> uint64
 val op_Less_Less_Hat:uint64 -> u32 -> uint64
 val op_Greater_Greater_Hat:uint64 -> u32 -> uint64
 val op_Amp_Hat:uint64 -> uint64 -> uint64
