crypto_hst/symmetric/Hacl.Symmetric.Poly1305.Bigint.fst
@@ -10,7 +10,7 @@ open Hacl.UInt64
 open Hacl.SBuffer
 open Math.Axioms
 open Math.Lib
-open Poly.Parameters
+open Hacl.Symmetric.Poly1305.Parameters
 
 #reset-options "--initial_fuel 0 --max_fuel 0"
 
