crypto_hst/symmetric/Hacl.Symmetric.Poly1305.Bignum.Lemmas.fst
@@ -1,0 +1,1495 @@
+module Hacl.Symmetric.Poly1305.Bignum.Lemmas
+
+open FStar.Mul
+open FStar.HyperStack
+open FStar.HST
+open FStar.Ghost
+open FStar.Buffer
+open Math.Axioms
+open Math.Lib
+open Math.Lemmas
+open Hacl.UInt64
+open Hacl.Cast
+open Hacl.SBuffer
+open Hacl.Symmetric.Poly1305.Parameters
+open Hacl.Symmetric.Poly1305.Bigint
+
+(* TODO, file not verified *)
+#reset-options "--lax"
+
+//TMP#reset-options "--initial_fuel 0 --max_fuel 0"
+
+(* Module abbreviations *)
+module HH = FStar.HyperHeap
+module HS = FStar.HyperStack
+
+module U8  = FStar.UInt8
+module U32 = FStar.UInt32
+module H8  = Hacl.UInt8
+module H32  = Hacl.UInt32
+module H64  = Hacl.UInt64
+
+(* This HAS to go in some more appropriate place *)
+assume MaxUInt8 : pow2 8 = 256
+assume MaxUInt32: pow2 32 = 4294967296
+assume MaxUInt64: pow2 64 > pow2 32
+
+//TMP#reset-options "--initial_fuel 4 --max_fuel 4"
+
+(* Prime value *)
+val prime: p:erased pos{reveal p = pow2 130 - 5}
+let prime = hide (pow2 130 - 5)
+
+//TMP#reset-options "--initial_fuel 0 --max_fuel 0"
+
+let live (h:heap) (b:bigint) : GTot Type0 = live h b /\ length b >= norm_length
+
+(* Lemmas that should go elsewhere but are terribly useful *)
+val distributivity_add_right: a:int -> b:int -> c:int -> Lemma (a*(b+c) = a * b + a * c)
+let distributivity_add_right a b c = ()
+val distributivity_add_left: a:int -> b:int -> c:int -> Lemma ((a+b)*c = a * c + b * c)
+let distributivity_add_left a b c = ()
+val paren_mul_left: a:int -> b:int -> c:int -> Lemma (a * b * c = ( a * b ) * c)
+let paren_mul_left a b c = ()
+val paren_mul_right: a:int -> b:int -> c:int -> Lemma (a * b * c = a * (b * c))
+let paren_mul_right a b c = ()
+val paren_add_left: a:int -> b:int -> c:int -> Lemma (a + b + c = ( a + b ) + c)
+let paren_add_left a b c = ()
+val paren_add_right: a:int -> b:int -> c:int -> Lemma (a + b + c = a + (b + c))
+let paren_add_right a b c = ()
+
+(*** Addition ***)
+
+let willNotOverflow (h:heap) (a_idx:nat) (b_idx:nat) (len:nat) (ctr:nat) (a:bigint) (b:bigint) : GTot Type0 =
+  live h a /\ length a >= a_idx+len /\ live h b /\ length b >= b_idx+len
+  /\ (forall (i:nat). {:pattern (v (get h a (i+a_idx)))} (i >= ctr /\ i < len) ==>
+	(v (get h a (i+a_idx)) + v (get h b (i+b_idx)) < pow2 64))
+
+let isNotModified (h0:heap) (h1:heap) (a_idx:nat) (len:nat) (ctr:nat) (a:bigint) : GTot Type0 = 
+  live h0 a /\ live h1 a /\ a_idx+len <= length a 
+  /\  (forall (i:nat). {:pattern (get h1 a i)} ((i<ctr+a_idx \/ i >= len+a_idx) /\ i < length a) ==>
+	       get h1 a i == get h0 a i)
+
+let isSum (h0:heap) (h1:heap) (a_idx:nat) (b_idx:nat) (len:nat) (ctr:nat) (a:bigint) (b:bigint) : GTot Type0 =
+  live h0 a /\ live h1 a /\ a_idx+len <= length a /\ live h0 b /\ b_idx+len <= length b
+  /\ (forall (i:nat). {:pattern (v (get h1 a (i+a_idx)))} (i>= ctr /\ i<len) ==> 
+	v (get h1 a (i+a_idx)) = v (get h0 a (i+a_idx)) + v (get h0 b (i+b_idx)))
+
+(* More specialized than the "no_upd_lemma_1" from FStar.Buffer.fst *)
+let eq_lemma_1 h0 h1 (a:bigint) (b:bigint) : Lemma 
+  (requires (modifies_1 a h0 h1 /\ disjoint a b /\ live h0 a /\ live h0 b))
+  (ensures  (live h0 b /\ live h1 b /\ (forall (i:nat). i < length b ==> get h1 b i == get h0 b i)))
+  = ()
+
+let eq_lemma_2 h0 h1 (a:bigint) (a':bigint) (b:bigint) : Lemma 
+  (requires (modifies_2 a a' h0 h1 /\ disjoint a b /\ disjoint a' b 
+    /\ live h0 a /\ live h0 b /\ live h0 a'))
+  (ensures  (live h0 b /\ live h1 b /\ (forall (i:nat). i < length b ==> get h1 b i == get h0 b i)))
+  = ()
+
+//TMP#reset-options "--initial_fuel 0 --max_fuel 0 --z3timeout 20"
+
+(* val fsum_index: a:bigint -> a_idx:u32 -> b:bigint{disjoint a b} -> b_idx:u32 -> len:u32 ->  *)
+(*   ctr:u32{U32.v ctr<=U32.v len} -> STL unit *)
+(*     (requires (fun h -> live h a /\ live h b /\ U32.v a_idx+U32.v len <= length a /\ U32.v b_idx+U32.v len <= length b *)
+(* 	(\* /\ willNotOverflow h (U32.v a_idx) (U32.v b_idx) (U32.v len) (U32.v ctr) a b)) *\) *)
+(* 	)) *)
+(*     (ensures (fun h0 _ h1 -> live h0 a /\ live h0 b /\ live h1 a /\ live h1 b *)
+(*       /\ U32.v a_idx+U32.v len <= length a /\ U32.v b_idx+U32.v len <= length b /\ modifies_1 a h0 h1 *)
+(*       (\* TODO: restore the functional correctness bits *\) *)
+(*       (\* /\ isNotModified h0 h1 (w a_idx) (w len) (w ctr) a *\) *)
+(*       (\* /\ isSum h0 h1 (w a_idx) (w b_idx) (w len) (w ctr) a b *\) *)
+(*     )) *)
+(* let rec fsum_index a a_idx b b_idx len ctr = *)
+(*   if U32 (len =^ ctr) then () *)
+(*   else begin *)
+(*       let i = ctr in *)
+(*       let (ai:Hacl.UInt64.t) = U32 a.(i+^a_idx) in *)
+(*       let (bi:Hacl.UInt64.t) = U32 b.(i+^b_idx) in *)
+(*       let z = ai +%^ bi in *)
+(*       a.(U32 (a_idx +^ i)) <- z; *)
+(*       fsum_index a a_idx b b_idx len (U32 (ctr +^ 1ul)); *)
+(*       () *)
+(*   end *)
+
+//TMP#reset-options "--initial_fuel 1 --max_fuel 1 --z3timeout 20"
+
+val addition_lemma: h0:heap -> h1:heap -> a:bigint{live h0 a /\ live h1 a} -> b:bigint{live h0 b} ->
+  len:nat{len <= length a /\ len <= length b /\ 
+	 (forall (i:nat). {:pattern (v (get h1 a i))} i < len ==> 
+	    v (get h1 a i) = v (get h0 a i) + v (get h0 b i)) } -> 
+  Lemma (requires (True)) (ensures (eval h0 a len + eval h0 b len = eval h1 a len))
+let rec addition_lemma h0 h1 a b len =
+  match len with
+  | 0 -> ()
+  | _ -> addition_lemma h0 h1 a b (len-1);
+    distributivity_add_right (pow2 (bitweight templ (len-1))) (v (get h0 a (len-1))) (v (get h0 b (len-1)))
+
+//TMP#reset-options "--initial_fuel 0 --max_fuel 0"
+
+(* val fsum': a:bigint -> b:bigint{disjoint a b} -> STL unit *)
+(*     (requires (fun h -> live h a /\ live h b *)
+(*       (\* norm h a /\ norm h b *\) *)
+(*     )) *)
+(*     (ensures (fun h0 u h1 -> live h0 a /\ live h0 b /\ live h1 a /\ modifies_1 a h0 h1 *)
+(*       (\* /\ norm h0 a /\ norm h0 b /\  *\) *)
+(*       (\* /\ eval h1 a norm_length = eval h0 a norm_length + eval h0 b norm_length *\) *)
+(*       (\* /\ isNotModified h0 h1 0 norm_length 0 a *\) *)
+(*       (\* /\ isSum h0 h1 0 0 norm_length 0 a b *\) *)
+(*     )) *)
+(* let fsum' a b = *)
+(*   fsum_index a 0ul b 0ul nlength 0ul; *)
+(*   () *)
+
+(* Scalar multiplication *)
+
+(* TODO *)
+//TMP#reset-options "--lax"
+
+val scalar_multiplication_lemma: h0:heap -> h1:heap -> a:bigint{live h0 a} ->
+  b:bigint{live h1 b} -> s:s64 -> len:nat{len <= length a /\ len <= length b} ->
+  Lemma
+    (requires (forall (i:nat). {:pattern (v (get h1 b i))} i < len ==> v (get h0 a i) * v s = v (get h1 b i)))
+    (ensures (eval h0 a len * v s = eval h1 b len))
+let rec scalar_multiplication_lemma h0 h1 a b s len =
+  match len with
+  | 0 -> ()
+  | _ ->
+    scalar_multiplication_lemma h0 h1 a b s (len-1);
+    eval_def h1 b len;
+    eval_def h0 a len;
+    cut (True /\ eval h1 b len = pow2 (bitweight templ (len-1)) * v (get h1 b (len-1)) + eval h1 b (len-1));
+    cut (True /\ eval h1 b len = pow2 (bitweight templ (len-1)) * v (get h0 a (len-1)) * v s + eval h0 a (len-1) * v s);
+    cut (True /\ eval h0 a len = pow2 (bitweight templ (len-1)) * v (get h0 a (len-1)) + eval h0 a (len-1));
+    distributivity_add_left (pow2 (bitweight templ (len-1)) * v (get h0 a (len-1))) (eval h0 a (len-1)) (v s);
+    paren_mul_left (pow2 (bitweight templ (len-1))) (v (get h0 a (len-1))) (v s)
+
+//TMP#reset-options "--initial_fuel 0 --max_fuel 0"
+
+let scalarProduct (h0:heap) (h1:heap) (ctr:nat) (a:bigint) (s:s64) (res:bigint) : GTot Type0 =
+  live h0 a /\ live h1 res /\ ctr <= norm_length
+  /\ (forall (i:nat). {:pattern (v (get h1 res i))} i < ctr ==> v (get h1 res i) = v (get h0 a i) * v s)
+
+(* Equality between fragments of buffers *)
+let equalSub (ha:heap) (a:bigint) (a_idx:nat) (hb:heap) (b:bigint) (b_idx:nat) (len:nat) : GTot Type0 =
+  (live ha a) /\ (live hb b) /\ (length a >= a_idx + len) /\ (length b >= b_idx + len)
+  /\ (forall (i:nat). {:pattern (get ha a (a_idx+i)) \/ (get hb b (b_idx+i))} i < len
+      ==> get ha a (a_idx+i) == get hb b (b_idx+i))
+
+let lemma_helper_01 (ctr:u32): Lemma (forall (i:nat). {:pattern (U32.v ctr+i-1)} U32.v ctr + i - 1 = U32.v ctr - 1 + i)
+  = ()
+
+let lemma_helper_02 h0 h2 (a:bigint{live h0 a}) (res:bigint{live h2 res}) (ctr:u32{U32.v ctr <= norm_length /\ U32.v ctr > 0}) (s:s64) : Lemma
+  (requires (
+    (forall (i:nat). {:pattern (v (get h2 res i))} i < U32.v ctr - 1 ==> v (get h2 res i) = v (get h0 a i) * v s)
+    /\ v (get h2 res (U32.v ctr - 1)) = v (get h0 a (U32.v ctr - 1)) * v s))
+  (ensures (scalarProduct h0 h2 (U32.v ctr) a s res))
+  = ()
+
+(* val scalar_multiplication_aux: res:bigint -> a:bigint{disjoint res a} -> s:s64 -> ctr:u32 -> STL unit *)
+(*   (requires (fun h -> live h res /\ live h a /\ U32.v ctr <= norm_length *)
+(*     (\* /\ (forall (i:nat). {:pattern (v (get h a i))} i < U32.v ctr ==> v (get h a i) * v s < poU32.v2 64)  *\) *)
+(*   )) *)
+(*   (ensures (fun h0 _ h1 -> live h1 res /\ modifies_1 res h0 h1 *)
+(*     (\* /\ scalarProduct h0 h1 (U32.v ctr) a s res  *\) *)
+(*     (\* /\ equal h0 a h1 a  *\) *)
+(*     (\* /\ equalSub h0 res (U32.v ctr) h1 res (U32.v ctr) (length res - U32.v ctr)  *\) *)
+(*   )) *)
+(* let rec scalar_multiplication_aux res a s ctr = *)
+(*   let open FStar.UInt32 in *)
+(*   if ctr =^ 0ul then () *)
+(*   else begin *)
+(*     let i = ctr -^ 1ul in *)
+(*     let ai = a.(i) in *)
+(*     let resi = H64 (ai *%^ s) in *)
+(*     res.(i) <- resi; *)
+(*     scalar_multiplication_aux res a s i; *)
+(*     () *)
+(*   end *)
+
+(* val scalar_multiplication: res:bigint -> a:bigint{disjoint res a} -> s:s64 -> STL unit *)
+(*   (requires (fun h -> live h res /\ live h a *)
+(*     (\* /\ (forall (i:nat). {:pattern (v (get h a i))} i < norm_length ==> v (get h a i) * v s < pow2 64)  *\) *)
+(*   )) *)
+(*   (ensures (fun h0 _ h1 -> live h1 res /\ modifies_1 res h0 h1 *)
+(*     (\* /\ scalarProduct h0 h1 norm_length a s res  *\) *)
+(*     (\* /\ equal h0 a h1 a  *\) *)
+(*     (\* /\ equalSub h0 res norm_length h1 res norm_length (length res - norm_length) *\) *)
+(*     (\* /\ eval h1 res norm_length = eval h0 a norm_length * v s  *\) *)
+(*   )) *)
+(* let scalar_multiplication res a s = *)
+(*   scalar_multiplication_aux res a s nlength; *)
+(*   () *)
+
+(* Multiplication *)
+
+//TMP#reset-options "--initial_fuel 1 --max_fuel 1"
+
+val bitweight_lemma_1: i:nat -> Lemma (bitweight templ i = i * templ 0)
+let rec bitweight_lemma_1 i =
+  match i with | 0 -> () | _ -> bitweight_lemma_1 (i-1)
+
+//TMP#reset-options "--initial_fuel 0 --max_fuel 0"
+
+val bitweight_lemma_0: i:nat -> j:nat ->
+  Lemma (bitweight templ (i+j) = bitweight templ i + bitweight templ j)
+let rec bitweight_lemma_0 i j =
+  bitweight_lemma_1 (i+j); bitweight_lemma_1 i; bitweight_lemma_1 j
+
+val auxiliary_lemma_1: a:nat -> b:nat ->
+  Lemma
+    (requires (True))
+    (ensures (pow2 (bitweight templ (a+b)) = pow2 (bitweight templ a) * pow2 (bitweight templ b)))
+let auxiliary_lemma_1 a b =
+  bitweight_lemma_0 a b;
+  Math.Lib.pow2_exp_lemma (bitweight templ a) (bitweight templ b);
+  ()
+
+let partialEquality (ha:heap) (a:bigint) (hb:heap) (b:bigint) (len:nat) : GTot Type0 =
+  live ha a /\ live hb b /\ len <= length a /\ len <= length b
+  /\ (forall (i:nat). {:pattern (v (get ha a i))} i < len ==> v (get ha a i) = v (get hb b i))
+
+let storesSum (hc:heap) (c:bigint) (ha:heap) (a:bigint) (hb:heap) (b:bigint)
+		      (a_idx:nat) (len:nat) : GTot Type0 =
+  live ha a /\ live hb b /\ live hc c /\ a_idx+len <= length a /\ len <= length b /\ a_idx+len <= length c
+  /\  (forall (i:nat). {:pattern (v (get hc c (i+a_idx)))}
+	(i < len ==> v (get hc c (i+a_idx)) = v (get ha a (i+a_idx)) + v (get hb b i)))
+
+val multiplication_step_lemma_1:
+  h0:heap -> h1:heap -> a:bigint{live h0 a} -> b:bigint{live h0 b} -> c:bigint{live h1 c} ->
+  idx:nat -> len:pos{len+idx <= length a /\ len <= length b /\ length a = length c} ->
+  Lemma
+    (requires (
+      (storesSum h1 c h0 a h0 b idx len)
+      /\ (partialEquality h1 c h0 a idx)
+      /\ (eval h1 c (len-1+idx) = eval h0 a (len-1+idx) + pow2 (bitweight templ idx) * eval h0 b (len-1))))
+    (ensures (eval h1 c (len+idx) = eval h0 a (len+idx) +
+		          pow2 (bitweight templ idx) * eval h0 b (len-1) +
+			  pow2 (bitweight templ (len-1+idx)) * v (get h0 b (len-1))))
+let multiplication_step_lemma_1 h0 h1 a b c idx len =
+  let t = templ in
+  cut (v (get h1 c (len+idx-1)) = v (get h0 a (len+idx-1)) + v (get h0 b (len-1)));
+  eval_def h1 c (len+idx);
+  cut (eval h1 c (len+idx) = pow2 (bitweight t (len+idx-1)) * v (get h1 c (len+idx-1)) + eval h1 c (len+idx-1));
+  cut (eval h1 c (len+idx) = eval h1 c (len+idx-1) + pow2 (bitweight t (len+idx-1)) * v (get h1 c (len+idx-1)));
+  cut (eval h1 c (len+idx-1) = eval h0 a (len+idx-1) + (pow2 (bitweight t idx)) * eval h0 b (len-1) /\ True);
+  cut (v (get h1 c (len+idx-1)) = v (get h0 a (len+idx-1)) + v (get h0 b (len-1)));
+  cut (eval h1 c (len+idx) =
+	(eval h0 a (len+idx-1) + (pow2 (bitweight t idx)) * eval h0 b (len-1))
+	+ pow2 (bitweight t (len-1+idx)) * (v (get h0 a (len+idx-1)) + v (get h0 b (len-1))));
+  distributivity_add_right (pow2 (bitweight t (len-1+idx))) (v (get h0 a (len+idx-1))) (v (get h0 b (len-1)));
+  cut (eval h1 c (len+idx) =
+	(eval h0 a (len+idx-1) + (pow2 (bitweight t idx)) * eval h0 b (len-1))
+	+ (pow2 (bitweight t (len-1+idx)) * v (get h0 a (len+idx-1))
+        + pow2 (bitweight t (len-1+idx)) * v (get h0 b (len-1))));
+  cut (eval h1 c (len+idx) =
+	eval h0 a (len+idx-1) + (pow2 (bitweight t idx)) * eval h0 b (len-1)
+	+ (pow2 (bitweight t (len-1+idx)) * v (get h0 a (len+idx-1))
+        + pow2 (bitweight t (len-1+idx)) * v (get h0 b (len-1))));
+  cut (eval h1 c (len+idx) = eval h0 a (len+idx-1) + pow2 (bitweight t idx) * eval h0 b (len-1)  +
+	  pow2 (bitweight t (len-1+idx)) * v (get h0 a (len+idx-1)) +
+          pow2 (bitweight t (len-1+idx)) * v (get h0 b (len-1)));
+  cut (eval h1 c (len+idx) =
+	pow2 (bitweight t (len-1+idx)) * v (get h0 a (len+idx-1)) + eval h0 a (len+idx-1) +
+          pow2 (bitweight t idx) * eval h0 b (len-1)  +
+          pow2 (bitweight t (len-1+idx)) * v (get h0 b (len-1)));
+  eval_def h0 a (len+idx);
+  cut (eval h0 a (len+idx) = pow2 (bitweight t (len+idx-1)) * v (get h0 a (len+idx-1)) + eval h0 a (len+idx-1));
+  cut (eval h1 c (len+idx) = eval h0 a (len+idx) + pow2 (bitweight t idx) * eval h0 b (len-1)
+		+ pow2 (bitweight t (len-1+idx)) * v (get h0 b (len-1)))
+
+val multiplication_step_lemma_2:
+  h0:heap -> h1:heap -> a:bigint{live h0 a} -> b:bigint{live h0 b} -> c:bigint{live h1 c} -> idx:nat ->
+  len:pos{len+idx <= length a /\ len <= length b /\ length a = length c} -> Lemma
+    (requires ( eval h1 c (len+idx) = eval h0 a (len+idx) +
+                          pow2 (bitweight templ idx) * eval h0 b (len-1)  +
+			  pow2 (bitweight templ (len-1+idx)) * v (get h0 b (len-1)) ))
+    (ensures (eval h1 c (len+idx) = eval h0 a (len+idx) + pow2 (bitweight templ idx) * eval h0 b len))
+let multiplication_step_lemma_2 h0 h1 a b c idx len =
+  auxiliary_lemma_1 idx (len-1);
+  cut (pow2 (bitweight templ (len-1+idx)) = pow2 (bitweight templ idx) * pow2 (bitweight templ (len-1)) );
+  paren_mul_left (pow2 (bitweight templ idx)) (pow2 (bitweight templ (len-1))) (v (get h0 b (len-1)));
+  cut (eval h1 c (len+idx) = eval h0 a (len+idx)
+			     + pow2 (bitweight templ idx) * eval h0 b (len-1)
+			     + pow2 (bitweight templ idx) * pow2 (bitweight templ (len-1)) * v (get h0 b (len-1)) /\ True);
+  distributivity_add_right (pow2 (bitweight templ idx)) (eval h0 b (len-1)) (pow2 (bitweight templ (len-1)) * v (get h0 b (len-1)));
+  eval_def h0 b len;
+  cut (eval h0 b len = eval h0 b (len-1) + (pow2 (bitweight templ (len-1))) * v (get h0 b (len-1)) );
+  cut (pow2 (bitweight templ (len-1+idx)) * v (get h0 b (len-1)) =
+        pow2 (bitweight templ idx) * pow2 (bitweight templ (len-1)) * v (get h0 b (len-1)));
+  cut ( eval h1 c (len+idx) = eval h0 a (len+idx) + pow2 (bitweight templ idx) * eval h0 b len)
+
+//TMP#reset-options "--initial_fuel 0 --max_fuel 0 --z3timeout 20"
+
+val multiplication_step_lemma:
+  h0:heap -> h1:heap -> a:bigint{live h0 a} -> b:bigint{live h0 b} -> c:bigint{live h1 c} -> idx:nat ->
+  len:nat{len+idx <= length a /\ len <= length b /\ length a = length c} -> Lemma
+    (requires (storesSum h1 c h0 a h0 b idx len /\ partialEquality h1 c h0 a idx))
+    (ensures (eval h1 c (len+idx) = eval h0 a (len+idx) + pow2 (bitweight templ idx) * eval h0 b len))
+let rec multiplication_step_lemma h0 h1 a b c idx len =
+  match len with
+  | 0 ->
+    cut (forall (i:nat). {:pattern (v (get h1 c i))} i < idx ==> v (get h1 c i) = v (get h0 a i));
+    eval_def h0 b 0;
+    eval_eq_lemma h0 h1 a c idx
+  | _ ->
+     multiplication_step_lemma h0 h1 a b c idx (len-1);
+     multiplication_step_lemma_1 h0 h1 a b c idx len;
+     multiplication_step_lemma_2 h0 h1 a b c idx len
+
+//TMP#reset-options "--initial_fuel 0 --max_fuel 0"
+
+let partialEquality2 (ha:heap) (a:bigint{live ha a}) (hb:heap) (b:bigint{live hb b})
+	             (len:nat) (len2:nat{len2 >= len /\ len2 <= length a /\ len2 <= length b}) : GTot Type0 =
+  (forall (i:nat). {:pattern (v (get ha a i))}  (i < len2 /\ i >= len) ==> v (get ha a i) = v (get hb b i))
+
+val auxiliary_lemma_5: h0:heap -> h1:heap -> a:bigint{live h0 a} ->
+  b:bigint{live h1 b} -> c:int -> len:nat -> len2:nat{len2 >= len /\ len2 <= length b /\ len2 <= length a} ->
+  Lemma
+    (requires (eval h1 b len = eval h0 a len + c /\ partialEquality2 h1 b h0 a len len2))
+    (ensures (eval h1 b len2 = eval h0 a len2 + c))
+let rec auxiliary_lemma_5 h0 h1 a b c len len2 =
+  match len2 - len with
+  | 0 -> ()
+  | _ ->
+     let t = templ in
+     auxiliary_lemma_5 h0 h1 a b c len (len2-1);
+     cut (eval h1 b (len2-1) = eval h0 a (len2-1) + c);
+     eval_def h1 b len2;
+     cut (eval h1 b len2 = eval h1 b (len2-1) + (pow2 (bitweight t (len2-1))) * v (get h1 b (len2-1)));
+     cut (v (get h1 b (len2-1)) = v (get h0 a (len2-1)) /\ True);
+     cut (eval h1 b len2 = (eval h0 a (len2-1) + c) + (pow2 (bitweight t (len2-1))) * v (get h0 a (len2-1)));
+     eval_def h0 a len2;
+     cut (eval h1 b len2 = eval h0 a len2 + c)
+
+let bound27 (h:heap) (b:bigint) : GTot Type0 =
+  live h b /\ length b >= norm_length
+  /\ (forall (i:nat). {:pattern (v (get h b i))} i < norm_length ==> v (get h b i) < pow2 27)
+
+(* val multiplication_step_0: a:bigint -> b:bigint -> ctr:u32{U32.v ctr<norm_length} -> c:bigint{disjoint a c /\ disjoint b c} -> tmp:bigint{disjoint a tmp /\ disjoint b tmp /\ disjoint c tmp} ->  STL unit *)
+(*      (requires (fun h -> live h a /\ live h b /\ live h c /\ live h tmp *)
+(*        (\* /\ bound27 h a /\ norm h b /\ live h c /\ live h tmp /\ length c >= 2*norm_length -1 *\) *)
+(*        (\* /\ maxValue h c (length c) <= w ctr * pow2 53 *\) *)
+(*      )) *)
+(*      (ensures (fun h0 _ h1 -> live h1 tmp /\ modifies_1 tmp h0 h1 *)
+(*        (\* /\ bound27 h0 a /\ norm h0 b /\ live h0 c /\ live h0 tmp /\ length c >= 2*norm_length-1 *\) *)
+(*        (\* /\ scalarProduct h0 h1 norm_length a (get h0 b (w ctr)) tmp *\) *)
+(*        (\* /\ eval h1 tmp norm_length = eval h0 a norm_length * v (get h0 b (w ctr)) *\) *)
+(*      )) *)
+(* let multiplication_step_0 a b ctr c tmp = *)
+(*   let s = b.(ctr) in *)
+(*   scalar_multiplication tmp a s *)
+
+val norm_lemma: h0:heap -> h1:heap -> a:bigint -> tmp:bigint{disjoint a tmp} -> Lemma
+    (requires (norm h0 a /\ live h0 tmp /\ modifies_1 tmp h0 h1))
+    (ensures (norm h1 a))
+let norm_lemma h0 h1 a tmp =
+  eq_lemma_1 h0 h1 tmp a;
+  ()
+
+val bound27_lemma: h0:heap -> h1:heap -> a:bigint -> tmp:bigint{disjoint a tmp} -> Lemma
+    (requires (bound27 h0 a /\ live h0 tmp /\ modifies_1 tmp h0 h1))
+    (ensures (bound27 h1 a))
+let bound27_lemma h0 h1 a tmp =
+  eq_lemma_1 h0 h1 tmp a;
+  ()
+
+//TMP#reset-options "--initial_fuel 4 --max_fuel 4"
+
+val aux_lemma_4: unit -> Lemma (pow2 3 = 8)
+let aux_lemma_4 () = ()
+
+//TMP#reset-options "--initial_fuel 0 --max_fuel 0"
+
+val aux_lemma_41: b:s64{v b < pow2 26} -> Lemma (forall (a:s64). (v a < pow2 27 /\ v b < pow2 26) ==> (v a * v b < pow2 53))
+let aux_lemma_41 b =
+  cut (forall (a:s64). v a < pow2 27 ==> v a * v b < pow2 27 * pow2 26);
+  Math.Lib.pow2_exp_lemma 27 26;
+  ()
+
+val aux_lemma_42: h:heap -> a:bigint{bound27 h a} -> z:s64{v z < pow2 26} -> Lemma (forall (i:nat). i < norm_length ==> v (get h a i) * v z < pow2 53)
+let aux_lemma_42 h a z =
+  cut (forall (i:nat). {:pattern (get h a i)} i < norm_length ==> (v (get h a i) < pow2 27));
+  aux_lemma_41 z;
+  Math.Lib.pow2_exp_lemma 27 26;
+  cut (forall (i:nat). i < norm_length ==> v (get h a i) * v z < pow2 53)
+
+val aux_lemma_43: h1:heap -> c:bigint{live h1 c /\ length c >= 2*norm_length-1} ->
+  tmp:bigint{live h1 tmp} -> ctr:nat{ctr < norm_length} -> Lemma
+  (requires ((forall (i:nat). {:pattern (v (get h1 tmp i))} i < norm_length ==> v (get h1 tmp i) < pow2 53)
+    /\ (forall (i:nat). {:pattern (v (get h1 c (i+ctr)))} i < norm_length ==> v (get h1 c (i+ctr)) <= ctr * pow2 53) ))
+	(ensures (forall (i:nat). {:pattern (v (get h1 c (i+ctr)) + v (get h1 tmp i))} i < norm_length ==> v (get h1 c (i+ctr)) + v (get h1 tmp i) <= (ctr+1) * pow2 53))
+let aux_lemma_43 h1 c tmp ctr =
+  ()
+
+//TMP#reset-options "--initial_fuel 4 --max_fuel 4"
+
+let lemma_helper_10 (x:nat) : Lemma (requires (x <= norm_length))
+				 (ensures  (x * pow2 53 <= pow2 3 * pow2 53))
+  = ()
+
+//TMP#reset-options "--initial_fuel 0 --max_fuel 0 --z3timeout 50"
+
+val multiplication_step_lemma_001: h0:heap -> h1:heap -> a:bigint -> b:bigint ->
+  ctr:nat{ctr<norm_length} -> c:bigint{disjoint a c /\ disjoint b c} ->
+  tmp:bigint{disjoint a tmp /\ disjoint b tmp /\ disjoint c tmp} ->
+  Lemma
+     (requires (
+       bound27 h0 a /\ norm h0 b /\ live h0 c /\ live h1 tmp /\ live h0 tmp
+       /\ (length c >= 2*norm_length -1)
+       /\ (maxValue h0 c (length c) <= ctr * pow2 53)
+       /\ modifies_1 tmp h0 h1
+       /\ scalarProduct h0 h1 norm_length a (get h0 b ctr) tmp ))
+     (ensures (live h1 c /\ live h1 tmp /\ ctr+norm_length <= length c
+       /\ willNotOverflow h1 ctr 0 norm_length 0 c tmp ))
+let multiplication_step_lemma_001 h0 h1 a b ctr c tmp =
+  eq_lemma_1 h0 h1 tmp c;
+  cut (live h1 c /\ v (get h0 b ctr) < pow2 (templ 0));
+  cut (forall (i:nat). {:pattern (get h1 c)} i < norm_length ==> i+ctr < length c);
+  cut (forall (i:nat). {:pattern (v (get h0 a i))} i < norm_length ==> (v (get h0 a i) < pow2 27));
+  cut (forall (i:nat). {:pattern (v (get h1 tmp i))} i < norm_length ==> v (get h1 tmp i) = v (get h0 a i) * v (get h0 b ctr));
+  Math.Lib.pow2_exp_lemma 27 26;
+  aux_lemma_42 h0 a (get h0 b ctr);
+  cut (forall (i:nat). {:pattern (v (get h1 tmp i))} i < norm_length ==> v (get h1 tmp i) < pow2 53);
+  maxValue_lemma h1 c;
+  maxValue_eq_lemma h0 h1 c c (length c);
+  cut (forall (i:nat). {:pattern (v (get h1 c (i+ctr)))} i < norm_length ==> v (get h1 c (i+ctr)) <= ctr * pow2 53);
+  aux_lemma_43 h1 c tmp ctr;
+  aux_lemma_4 ();
+  lemma_helper_10 (ctr+1);
+  Math.Lib.pow2_exp_lemma 3 53;
+  Math.Lib.pow2_increases_lemma 64 56;
+  cut((ctr+1) * pow2 53 < pow2 platform_wide);
+  cut (forall (i:nat). (i < norm_length /\ i >= 0) ==> v (get h1 c (i+ctr)) + v (get h1 tmp (i+0)) < pow2 64)
+
+//TMP#reset-options "--initial_fuel 0 --max_fuel 0"
+
+val aux_lemma_5: ctr:nat -> Lemma (ctr * pow2 53 <= (ctr+1) * pow2 53)
+let aux_lemma_5 ctr = ()
+
+val aux_lemma_51: ctr:nat -> Lemma (ctr * pow2 53 + pow2 53 = (ctr+1) * pow2 53)
+let aux_lemma_51 ctr = ()
+
+let lemma_helper_20 () : Lemma  (forall (a:nat) (b':nat) (c:nat) (d:nat). (a < c /\ b' < d) ==> a * b' < c * d)
+  = ()
+
+//TMP#reset-options "--initial_fuel 0 --max_fuel 0 --z3timeout 50"
+
+val max_value_lemma_1: h0:heap -> h1:heap -> h2:heap -> a:bigint -> b:bigint ->
+  ctr:nat{ctr < norm_length} -> c:bigint{disjoint a c /\ disjoint b c} ->
+  tmp:bigint{disjoint a tmp /\ disjoint b tmp /\ disjoint c tmp} -> Lemma
+    (requires (
+      bound27 h0 a /\ norm h0 b /\ live h0 c /\ live h1 tmp /\ live h2 c /\ live h1 c
+      /\ modifies_1 tmp h0 h1 /\ length c >= 2 * norm_length - 1
+      /\ (maxValue h0 c (length c) <= ctr * pow2 53)
+      /\ (forall (i:nat). {:pattern (v (get h2 c (i+ctr)))}
+	  i < norm_length ==> v (get h2 c (i+ctr)) = v (get h0 c (i+ctr)) + (v (get h0 a i) * v (get h0 b ctr)))
+      /\ (forall (i:nat). {:pattern (v (get h2 c i))} ((i < ctr \/ i >= norm_length + ctr) /\ i < length c) ==> v (get h2 c i) = v (get h0 c i)) ))
+    (ensures (bound27 h0 a /\ norm h0 b /\ live h2 c /\ maxValue h2 c (length c) <= (ctr+1) * pow2 53 ))
+let max_value_lemma_1 h0 h1 h2 a b ctr c tmp =
+  cut(forall (i:nat). {:pattern (v (get h0 a i))} i < norm_length ==> v (get h0 a i) < pow2 27);
+  cut(forall (i:nat). {:pattern (v (get h0 b i))} i < norm_length ==> v (get h0 b i) < pow2 26);
+  maxValue_lemma h0 c;
+  cut (forall (i:nat). {:pattern (v (get h0 c i))} i < length c ==> v (get h0 c i) <= maxValue h0 c (length c)) ;
+  cut (forall (i:nat). {:pattern (v (get h0 c (i+ctr)))} i < norm_length ==> v (get h0 c (i+ctr)) <= maxValue h0 c (length c));
+  lemma_helper_20 ();
+  aux_lemma_42 h0 a (get h0 b ctr);
+  cut (forall (i:nat). {:pattern (v (get h0 a i) * v (get h0 b ctr))} i < norm_length ==>
+    v (get h0 a i) * v (get h0 b ctr) < pow2 53);
+  cut (forall (i:nat). {:pattern (v (get h0 c (i+ctr)) + (v (get h0 a i) * v (get h0 b ctr)))} i < norm_length ==> v (get h0 c (i+ctr)) + (v (get h0 a i) * v (get h0 b ctr)) <= ctr * pow2 53 + pow2 53);
+  aux_lemma_51 ctr;
+  cut (forall (i:nat). {:pattern (v (get h2 c (i+ctr)))} i < norm_length ==> v (get h2 c (i+ctr)) <= (ctr+1) * pow2 53);
+  cut (forall (i:nat). (i >= ctr /\ i < norm_length + ctr) ==> v (get h2 c (i-ctr+ctr)) <= (ctr+1) * pow2 53);
+  cut (forall (i:nat). {:pattern (v (get h2 c i))} ((i < ctr \/ i >= norm_length+ctr) /\ i < length c) ==> v (get h2 c i) <= ctr * pow2 53);
+  aux_lemma_5 ctr;
+  cut (forall (i:nat). i < length c ==> v (get h2 c i) <= (ctr+1) * pow2 53);
+  maxValue_bound_lemma h2 c ((ctr+1) * pow2 53)
+
+//TMP#reset-options "--initial_fuel 0 --max_fuel 0"
+
+let eq_lemma_0 h0 h1 (a:bigint) : Lemma
+  (requires (modifies_0 h0 h1 /\ live h0 a))
+  (ensures  (live h0 a /\ live h1 a /\ (forall (i:nat). i < length a ==> get h1 a i == get h0 a i)))
+  = ()
+
+(* TODO *)
+//TMP#reset-options "--lax"
+
+val max_value_lemma: h0:heap -> h1:heap -> h2:heap -> a:bigint -> b:bigint ->
+  ctr:nat{ctr < norm_length} -> c:bigint{disjoint a c /\ disjoint b c} ->
+  tmp:bigint{disjoint a tmp /\ disjoint b tmp /\ disjoint c tmp} ->  Lemma
+    (requires (
+      bound27 h0 a /\ norm h0 b /\ live h0 c /\ live h1 tmp /\ live h2 c /\ live h1 c /\ live h0 tmp
+      /\ modifies_1 tmp h0 h1 /\ length c >= 2 * norm_length - 1
+      /\ maxValue h0 c (length c) <= ctr * pow2 53
+      /\ scalarProduct h0 h1 norm_length a (get h0 b ctr) tmp
+      /\ isSum h1 h2 ctr 0 norm_length 0 c tmp
+      /\ equalSub h1 c 0 h2 c 0 ctr
+      /\ equalSub h1 c (norm_length+ctr) h2 c (norm_length+ctr) (length c - norm_length - ctr) ))
+    (ensures (bound27 h0 a /\ norm h0 b /\ live h2 c /\ maxValue h2 c (length c) <= (ctr+1) * pow2 53))
+let max_value_lemma h0 h1 h2 a b ctr c tmp =
+  cut(forall (i:nat). {:pattern (v (get h1 tmp i))} i < norm_length ==> v (get h1 tmp i) = v (get h0 a i) * v (get h0 b ctr));
+  cut(forall (i:nat). {:pattern (v (get h2 c (i+ctr)))} i < norm_length ==> v (get h2 c (i+ctr)) = v (get h1 c (i+ctr)) + v (get h1 tmp (i+0)));
+  cut (forall (i:nat). {:pattern (v (get h2 c i))} i < ctr ==> v (get h2 c (0+i)) = v (get h1 c (0+i)));
+  cut (forall (i:nat). {:pattern (v (get h2 c i))} i < length c - norm_length - ctr ==> v (get h2 c ((norm_length+ctr)+i)) = v (get h1 c ((norm_length+ctr)+i)));
+  eq_lemma_1 h0 h1 tmp c;
+  cut (forall (i:nat). {:pattern (v (get h1 c i))} i < length c ==> v (get h1 c i) = v (get h0 c i));
+  cut (forall (i:nat). {:pattern (v (get h1 tmp i))}
+    i < norm_length ==> v (get h1 tmp i) = v (get h0 a i) * v (get h0 b ctr));
+  cut(forall (i:nat). i < norm_length ==> v (get h2 c (i+ctr)) = v (get h0 c (i+ctr)) + v (get h0 a (i+0)) * v (get h0 b ctr));
+  cut (forall (i:nat). {:pattern (v (get h2 c i))} (i >= norm_length + ctr /\ i < length c) ==> v (get h2 c ((norm_length+ctr)+(i-norm_length-ctr))) = v (get h0 c ((norm_length+ctr)+(i-norm_length-ctr))));
+  cut (forall (i:nat). {:pattern (v (get h2 c i))} i < ctr ==> v (get h2 c (0+i)) = v (get h0 c (0+i)));
+  cut (forall (i:nat). {:pattern (v (get h2 c i))} (i >=norm_length + ctr /\ i < length c) ==> v (get h2 c i) = v (get h0 c i));
+  cut (forall (i:nat). {:pattern (v (get h2 c i))} i < ctr ==> v (get h2 c i) = v (get h0 c i));
+  max_value_lemma_1 h0 h1 h2 a b ctr c tmp
+
+//TMP#reset-options "--max_fuel 0 --initial_fuel 0"
+
+let lemma_modifies_2_refl a b h0 h1 : Lemma (requires (modifies_2 a b h0 h1))
+					    (ensures  (modifies_2 b a h0 h1))
+  = ()
+
+val standardized_lemma: h0:heap -> h1:heap -> h2:heap -> a:bigint -> c:bigint{disjoint a c} ->
+  tmp:bigint{disjoint a tmp /\ disjoint c tmp} -> Lemma
+    (requires (bound27 h0 a /\ live h0 c /\ live h1 tmp /\ live h1 c /\ modifies_1 tmp h0 h1
+      /\ live h0 tmp /\ (modifies_1 c h1 h2) ))
+     (ensures (bound27 h0 a /\ bound27 h2 a /\ live h0 c /\ live h1 tmp /\ live h2 tmp
+       /\ modifies_2 c tmp h0 h2))
+let standardized_lemma h0 h1 h2 a c tmp =
+  eq_lemma_1 h1 h2 c tmp;
+  eq_lemma_1 h0 h1 tmp c;
+  lemma_modifies_1_1 tmp c h0 h1 h2;
+  lemma_modifies_2_refl tmp c h0 h2;
+  assert(modifies_2 tmp c h0 h2);
+  eq_lemma_2 h0 h2 c tmp a;
+  ()
+
+val standardized_lemma2: h0:heap -> h1:heap -> h2:heap -> a:bigint -> c:bigint{disjoint a c} ->
+  tmp:bigint{disjoint a tmp /\ disjoint c tmp} -> Lemma
+    (requires (norm h0 a /\ live h0 c /\ live h0 tmp /\ live h1 tmp /\ live h1 c /\ modifies_1 tmp h0 h1
+	/\ (modifies_1 c h1 h2) ))
+     (ensures (norm h0 a /\ norm h2 a /\ live h0 c /\ live h1 tmp /\ live h2 tmp
+       /\ modifies_2 c tmp h0 h2))
+let standardized_lemma2 h0 h1 h2 a c tmp =
+  eq_lemma_1 h1 h2 c tmp;
+  eq_lemma_1 h0 h1 tmp c;
+  lemma_modifies_1_1 tmp c h0 h1 h2;
+  lemma_modifies_2_refl tmp c h0 h2;
+  assert(modifies_2 tmp c h0 h2);
+  eq_lemma_2 h0 h2 c tmp a;
+  ()
+
+(* TODO *)
+//TMP#reset-options "--lax"
+
+val multiplication_step_lemma_02: h0:heap -> h1:heap -> h2:heap -> a:bigint -> b:bigint ->
+  ctr:nat{ctr<norm_length} -> c:bigint{disjoint a c /\ disjoint b c} ->
+  tmp:bigint{disjoint a tmp /\ disjoint b tmp /\ disjoint c tmp} -> Lemma
+     (requires (bound27 h0 a /\ norm h0 b /\ live h0 c /\ live h1 tmp /\ live h1 c /\ live h0 tmp
+	/\ length c >= 2 * norm_length - 1
+	/\ maxValue h0 c (length c) <= ctr * pow2 53
+	// After fscalar
+	/\ modifies_1 tmp h0 h1
+	/\ scalarProduct h0 h1 norm_length a (get h0 b ctr) tmp
+        /\ eval h1 tmp norm_length = eval h0 a norm_length * v (get h0 b ctr)
+ 	// After fsum
+	/\ live h2 c /\ live h2 tmp
+	/\ modifies_1 c h1 h2
+	/\ isSum h1 h2 ctr 0 norm_length 0 c tmp
+	/\ equalSub h1 c 0 h2 c 0 ctr
+	/\ equalSub h1 c (norm_length+ctr) h2 c (norm_length+ctr) (length c - norm_length - ctr)
+	))
+     (ensures (bound27 h0 a /\ norm h0 b /\ live h0 c /\ live h2 c  /\ live h0 tmp /\ live h2 tmp
+       /\ bound27 h2 a /\ norm h2 b
+       /\ length c >= 2 * norm_length - 1 /\ modifies_2 c tmp h0 h2
+       /\ (maxValue h2 c (length c) <= (ctr+1) * pow2 53)
+       /\ (eval h2 c (2*norm_length-1) = eval h0 c (2*norm_length-1) + pow2 (bitweight templ ctr) * eval h0 a norm_length * v (get h0 b ctr)) ))
+let multiplication_step_lemma_02 h0 h1 h2 a b ctr c tmp =
+  cut (forall (i:nat). {:pattern (v (get h1 c i))} i < ctr ==> v (get h1 c (0+i)) = v (get h2 c (0+i)));
+  cut (forall (i:nat). i < ctr ==> v (get h1 c i) = v (get h2 c i));
+  cut (partialEquality h2 c h1 c ctr);
+  cut (forall (i:nat). i < length c - norm_length - ctr ==> v (get h1 c ((norm_length+ctr)+i)) = v (get h2 c ((norm_length+ctr)+i)));
+  eval_partial_eq_lemma h1 h2 c c (norm_length+ctr) (2*norm_length-1);
+  eq_lemma_1 h0 h1 tmp c;
+  cut (forall (i:nat). i < 2*norm_length-1 ==> get h1 c i == get h0 c i);
+  eval_eq_lemma h0 h1 c c (2*norm_length-1);
+  eval_eq_lemma h0 h1 c c (norm_length+ctr);
+  cut (eval h2 c (2*norm_length-1) - eval h2 c (norm_length+ctr) = eval h0 c (2*norm_length-1) - eval h0 c (norm_length+ctr));
+  cut (eval h1 tmp norm_length = eval h0 a norm_length * v (get h0 b ctr));
+  cut (storesSum h2 c h1 c h1 tmp ctr norm_length);
+  multiplication_step_lemma h1 h2 c tmp c ctr norm_length;
+  eval_def h2 c (norm_length+ctr);
+  cut (eval h2 c (norm_length+ctr) = eval h1 c (norm_length+ctr) + pow2 (bitweight templ ctr) * eval h0 a norm_length * v (get h0 b ctr));
+  cut (eval h2 c (norm_length+ctr) = eval h0 c (norm_length+ctr) + pow2 (bitweight templ ctr) * eval h0 a norm_length * v (get h0 b ctr));
+  cut (eval h2 c (2*norm_length-1) = eval h0 c (2*norm_length-1) + pow2 (bitweight templ ctr) * eval h0 a norm_length * v (get h0 b ctr));
+  max_value_lemma h0 h1 h2 a b ctr c tmp;
+  cut (maxValue h2 c (length c) <= (ctr+1) * pow2 53);
+  standardized_lemma h0 h1 h2 a c tmp;
+  standardized_lemma2 h0 h1 h2 b c tmp
+
+//TMP#reset-options "--initial_fuel 0 --max_fuel 0"
+
+let lemma_helper_70 h0 h1 ctr (c:bigint{length c >= norm_length + U32.v ctr}) : Lemma
+  (requires (isNotModified h0 h1 (U32.v ctr) norm_length 0 c))
+  (ensures  (equalSub h0 c 0 h1 c 0 (U32.v ctr)
+    /\ equalSub h0 c (norm_length+U32.v ctr) h1 c (norm_length+U32.v ctr) (length c - norm_length - U32.v ctr) ))
+  = ()
+
+(* val multiplication_step_p1: a:bigint -> b:bigint -> ctr:u32{U32.v ctr<norm_length} -> *)
+(*   c:bigint{disjoint a c /\ disjoint b c /\ length c >= 2*norm_length-1} -> *)
+(*   tmp:bigint{disjoint a tmp /\ disjoint b tmp /\ disjoint c tmp} ->  STL unit *)
+(*      (requires (fun h -> live h a /\ live h b /\ live h c /\ live h tmp *)
+(* 	(\* /\ bound27 h a /\ norm h b *\) *)
+(*         (\* /\ (maxValue h c (length c) <= U32.v ctr * pow2 53) *\) *)
+(* 	(\* /\ (eval h c (2*norm_length-1) = eval h a (norm_length) * eval h b (U32.v ctr)) *\) *)
+(*      )) *)
+(*      (ensures (fun h0 u h1 -> live h1 c /\ live h1 tmp /\ modifies_2 c tmp h0 h1 *)
+(*        (\* (bound27 h0 a) /\ (norm h0 b) /\ (live h0 c) /\ (live h0 tmp) *\) *)
+(*        (\* /\ (bound27 h1 a) /\ (norm h1 b) *\) *)
+(*        (\* /\ (maxValue h0 c (length c) <= U32.v ctr * pow2 53) *\) *)
+(*        (\* /\ (maxValue h1 c (length c) <= (U32.v ctr+1) * pow2 53) *\) *)
+(*        (\* /\ (eval h0 c (2*norm_length-1) = eval h0 a (norm_length) * eval h0 b (U32.v ctr)) *\) *)
+(*        (\* /\ (eval h1 c (2*norm_length-1) = eval h0 c (2*norm_length-1) + pow2 (bitweight templ (U32.v ctr)) * eval h0 a norm_length * v (get h0 b (U32.v ctr))) *\) *)
+(*      )) *)
+(* let multiplication_step_p1 a b ctr c tmp = *)
+(*   multiplication_step_0 a b ctr c tmp; *)
+(*   fsum_index c ctr tmp 0ul nlength 0ul *)
+
+let helper_lemma_61 (a:int) (b:int) (c:int) (d:int) : Lemma (a*b*c+d = d+c*a*b) = ()
+
+val helper_lemma_6: h0:heap -> h1:heap -> a:bigint -> b:bigint -> ctr:nat{ctr < norm_length} ->
+  c:bigint{disjoint a c /\ disjoint b c /\ length c >= 2 * norm_length - 1} ->
+  tmp:bigint{disjoint a tmp /\ disjoint b tmp /\ disjoint c tmp} -> Lemma
+     (requires (bound27 h0 a /\ norm h0 b /\ live h0 c))
+    (ensures (bound27 h0 a /\ norm h0 b /\ live h0 c
+       /\ eval h0 c (2*norm_length-1) + pow2 (bitweight templ ctr) * eval h0 a (norm_length) * v (get h0 b ctr)  = eval h0 a (norm_length) * v (get h0 b ctr) * pow2 (bitweight templ ctr) + eval h0 c (2*norm_length-1) ))
+let helper_lemma_6 h0 h1 a b ctr c tmp =
+  helper_lemma_61 (eval h0 a norm_length) (v (get h0 b ctr)) (pow2 (bitweight templ ctr)) (eval h0 c (2*norm_length-1))
+
+(* val multiplication_step: a:bigint -> b:bigint -> ctr:u32{U32.v ctr < norm_length} -> *)
+(*   c:bigint{disjoint a c /\ disjoint b c /\ length c >= 2*norm_length-1} -> *)
+(*   tmp:bigint{disjoint a tmp /\ disjoint b tmp /\ disjoint c tmp} -> STL unit *)
+(*      (requires (fun h ->  live h a  /\ live h b /\ live h c /\ live h tmp *)
+(*         (\* /\ bound27 h a /\ norm h b *\) *)
+(* 	(\* /\ maxValue h c (length c) <= U32.v ctr * pow2 53 *\) *)
+(* 	(\* /\ eval h c (2*norm_length-1) = eval h a (norm_length) * eval h b (U32.v ctr) *\) *)
+(*      )) *)
+(*      (ensures (fun h0 u h1 -> live h1 c /\ live h1 tmp /\ modifies_2 c tmp h0 h1 *)
+(*        (\* /\ bound27 h0 a /\ bound27 h1 a /\ norm h0 b /\ norm h1 b *\) *)
+(*        (\* /\ live h0 c /\ live h1 c  /\ live h0 tmp *\) *)
+(*        (\* /\ maxValue h0 c (length c) <= U32.v ctr * pow2 53 *\) *)
+(*        (\* /\ maxValue h1 c (length c) <= (U32.v ctr+1) * pow2 53 *\) *)
+(*        (\* /\ eval h0 c (2*norm_length-1) = eval h0 a (norm_length) * eval h0 b (U32.v ctr) *\) *)
+(*        (\* /\ eval h1 c (2*norm_length-1) = eval h0 a (norm_length) * v (get h0 b (U32.v ctr)) * pow2 (bitweight templ (U32.v ctr)) + eval h0 c (2*norm_length-1) *\) *)
+(*      )) *)
+(* let multiplication_step a b ctr c tmp = *)
+(*   multiplication_step_p1 a b ctr c tmp *)
+
+//TMP#reset-options "--initial_fuel 1 --max_fuel 1 --z3timeout 20"
+
+val multiplication_step_lemma_03: h0:heap -> h1:heap -> a:bigint{norm h0 a} ->
+  b:bigint{norm h0 b} -> ctr:pos{ctr<=norm_length} ->
+  c:bigint{live h1 c /\ length c >= 2*norm_length-1} -> Lemma
+    (requires (eval h1 c (2*norm_length-1) = (eval h0 a (norm_length) * v (get h0 b (norm_length - ctr))) * pow2 (bitweight templ (norm_length - ctr)) + eval h0 a (norm_length) * eval h0 b (norm_length - ctr) ))
+    (ensures ( eval h1 c (2*norm_length-1) = eval h0 a (norm_length) * eval h0 b (norm_length - ctr + 1)))
+let multiplication_step_lemma_03 h0 h1 a b ctr c =
+  let t = templ in
+  paren_mul_left (eval h0 a norm_length) (v (get h0 b (norm_length - ctr))) (pow2 (bitweight t (norm_length - ctr)));
+  cut (eval h1 c (2*norm_length-1) = eval h0 a norm_length * v (get h0 b (norm_length - ctr)) * pow2 (bitweight t (norm_length - ctr)) + eval h0 a norm_length * eval h0 b (norm_length - ctr) );
+  cut (eval h1 c (2*norm_length-1) = eval h0 a norm_length * pow2 (bitweight t (norm_length - ctr)) * v (get h0 b (norm_length - ctr)) + eval h0 a norm_length * eval h0 b (norm_length - ctr) );
+  distributivity_add_right (eval h0 a norm_length) (pow2 (bitweight t (norm_length - ctr)) * v (get h0 b (norm_length - ctr))) (eval h0 b (norm_length - ctr));
+  cut (eval h1 c (2*norm_length-1) = eval h0 a norm_length * (pow2 (bitweight t (norm_length - ctr)) * v (get h0 b (norm_length - ctr)) + eval h0 b (norm_length - ctr)))
+
+//TMP#reset-options "--initial_fuel 0 --max_fuel 0"
+
+val helper_lemma_12: a:nat -> v:nat -> p:nat -> b:nat -> Lemma (a * v * p + (a * b) = a * (p * v + b))
+let helper_lemma_12 a v p b = ()
+
+(* TODO *)
+//TMP#reset-options "--lax"
+
+val multiplication_aux_lemma: h0:heap -> h1:heap -> a:bigint -> b:bigint ->
+  ctr:pos{ctr <= norm_length} ->  c:bigint{disjoint a c /\ disjoint b c} ->
+  tmp:bigint{disjoint a tmp /\ disjoint b tmp /\ disjoint c tmp} -> Lemma
+    (requires (bound27 h0 a /\ bound27 h1 a /\ norm h0 b /\ norm h1 b
+       /\ live h0 c /\ live h1 c /\ live h0 tmp /\ live h1 tmp
+       /\ length c >= 2 * norm_length - 1 /\ modifies_2 c tmp h0 h1
+       /\ maxValue h0 c (length c) <= (norm_length - ctr) * pow2 53
+       /\ maxValue h1 c (length c) <= ((norm_length - ctr)+1) * pow2 53
+       /\ eval h0 c (2*norm_length-1) = eval h0 a (norm_length) * eval h0 b (norm_length - ctr)
+       /\ eval h1 c (2*norm_length-1) = eval h0 a (norm_length) * v (get h0 b (norm_length - ctr)) * pow2 (bitweight templ (norm_length - ctr)) + eval h0 c (2*norm_length-1) ))
+    (ensures (bound27 h1 a /\ norm h1 b /\ live h1 c /\ live h1 tmp
+	/\ length c >= 2 * norm_length - 1
+	/\ maxValue h1 c (length c) <= (norm_length - ctr + 1) * pow2 53
+	/\ eval h1 c (2*norm_length-1) = eval h1 a (norm_length) * eval h1 b (norm_length - ctr + 1) ))
+let multiplication_aux_lemma h0 h1 a b ctr c tmp =
+  eq_lemma_2 h0 h1 c tmp a;
+  eq_lemma_2 h0 h1 c tmp b;
+  eval_eq_lemma h0 h1 a a norm_length;
+  eval_eq_lemma h0 h1 b b norm_length;
+  eval_eq_lemma h0 h1 b b (norm_length - ctr);
+  eval_eq_lemma h0 h1 b b (norm_length - ctr + 1);
+  cut((norm_length - ctr)+1 = norm_length - ctr + 1);
+  cut(eval h0 a norm_length = eval h1 a norm_length);
+  cut(eval h0 b (norm_length-ctr) = eval h1 b (norm_length - ctr));
+  cut(eval h0 b (norm_length - ctr + 1) = eval h1 b (norm_length - ctr + 1));
+  cut(v (get h0 b (norm_length - ctr)) = v (get h1 b (norm_length - ctr)));
+  helper_lemma_12 (eval h0 a norm_length) (v (get h0 b (norm_length - ctr))) (pow2 (bitweight templ (norm_length - ctr))) (eval h0 b (norm_length - ctr))
+
+val multiplication_aux_lemma_2: h0:heap -> h1:heap -> h2:heap -> a:bigint -> b:bigint ->
+  ctr:nat{ctr <= norm_length} -> c:bigint{disjoint a c /\ disjoint b c /\ length c >= 2*norm_length-1} ->
+  tmp:bigint{disjoint a tmp /\ disjoint b tmp /\ disjoint c tmp} -> Lemma
+    (requires (bound27 h0 a /\ norm h0 b /\ live h1 c /\ live h1 tmp /\ live h0 tmp /\ live h0 c
+       /\ bound27 h1 a /\ norm h1 b /\ live h1 c /\ live h1 tmp
+       /\ bound27 h2 a /\ norm h2 b /\ live h2 c /\ live h2 tmp
+       /\ modifies_2 c tmp h1 h2 /\ modifies_2 c tmp h0 h1
+       /\ eval h2 c (2*norm_length-1) = eval h1 a (norm_length) * eval h1 b (norm_length) ))
+    (ensures (bound27 h0 a /\ norm h0 b /\ live h1 c /\ bound27 h2 a /\ norm h2 b /\ live h2 c
+       /\ modifies_2 c tmp h0 h2
+       /\ eval h2 c (2*norm_length-1) = eval h0 a (norm_length) * eval h0 b (norm_length) ))
+let multiplication_aux_lemma_2 h0 h1 h2 a b ctr c tmp =
+  lemma_modifies_2_trans c tmp h0 h1 h2;
+  eq_lemma_2 h0 h1 c tmp a;
+  eq_lemma_2 h0 h1 c tmp b;
+  eval_eq_lemma h0 h1 a a norm_length;
+  eval_eq_lemma h0 h1 b b norm_length
+
+
+//TMP#reset-options "--initial_fuel 0 --max_fuel 0"
+
+(* val multiplication_aux: a:bigint -> b:bigint -> ctr:u32{U32.v ctr<=norm_length} -> *)
+(*   c:bigint{disjoint a c /\ disjoint b c /\ length c >= 2*norm_length-1} -> *)
+(*   tmp:bigint{disjoint a tmp /\ disjoint b tmp /\ disjoint c tmp} -> STL unit *)
+(*      (requires (fun h -> live h a /\ live h b  /\ live h c /\ live h tmp *)
+(*         (\* /\ bound27 h a /\ norm h b *\) *)
+(* 	(\* /\ maxValue h c (length c) <= (norm_length - U32.v ctr) * pow2 53 *\) *)
+(* 	(\* /\ eval h c (2*norm_length-1) = eval h a (norm_length) * eval h b (norm_length - U32.v ctr) *\) *)
+(*      )) *)
+(*      (ensures (fun h0 u h1 -> live h1 c /\ live h1 tmp /\ modifies_2 c tmp h0 h1 *)
+(*        (\* /\ bound27 h0 a /\ norm h0 b /\ live h0 c /\ live h0 tmp *\) *)
+(*        (\* /\ bound27 h1 a /\ norm h1 b *\) *)
+(*        (\* /\ eval h1 c (2*norm_length-1) = eval h0 a (norm_length) * eval h0 b (norm_length) *\) *)
+(*        (\* /\ maxValue h1 c (length c) <= norm_length * pow2 53 *\) *)
+(*      )) *)
+(* let rec multiplication_aux a b ctr c tmp = *)
+(*   let open FStar.UInt32 in *)
+(*   if ctr =^ 0ul then () *)
+(*   else begin *)
+(*     multiplication_step a b (nlength -^ ctr) c tmp; *)
+(*     multiplication_aux a b (ctr -^ 1ul) c tmp *)
+(*   end *)
+
+val helper_lemma_13: h0:heap -> h1:heap -> a:bigint ->
+  Lemma
+    (requires (bound27 h0 a /\ modifies_0 h0 h1))
+    (ensures (bound27 h0 a /\ bound27 h1 a /\ live h1 a /\ eval h0 a norm_length = eval h1 a norm_length))
+let helper_lemma_13 h0 h1 a =
+  eq_lemma_0 h0 h1 a;
+  eval_eq_lemma h0 h1 a a norm_length;
+  ()
+
+val helper_lemma_131: h0:heap -> h1:heap -> a:bigint ->
+  Lemma
+    (requires (norm h0 a /\ modifies_0 h0 h1))
+    (ensures (norm h0 a /\ norm h1 a /\ live h1 a /\ eval h0 a norm_length = eval h1 a norm_length))
+let helper_lemma_131 h0 h1 a =
+  eq_lemma_0 h0 h1 a;
+  eval_eq_lemma h0 h1 a a norm_length;
+  ()
+
+val helper_lemma_15: h0:heap -> h1:heap -> c:bigint{length c >= 2*norm_length-1} -> Lemma
+    (requires (live h0 c /\ null h0 c /\ modifies_0 h0 h1))
+    (ensures (live h1 c /\ null h1 c /\ maxValue h1 c (length c) = 0 /\ eval h1 c (2*norm_length-1) = 0))
+let helper_lemma_15 h0 h1 c =
+  eq_lemma_0 h0 h1 c;
+  eval_null h1 c (2*norm_length - 1);
+  max_value_of_null_lemma h1 c (length c)
+
+val multiplication_lemma_1: h0:heap -> h1:heap -> c:bigint{length c >= 2*norm_length-1} ->
+  a:bigint{disjoint c a} ->  b:bigint{disjoint c b} -> Lemma
+     (requires (bound27 h0 a /\ norm h0 b /\ live h0 c /\ null h0 c /\ modifies_0 h0 h1))
+     (ensures (bound27 h1 a /\ norm h1 b /\ live h1 c /\ null h1 c
+	/\ maxValue h1 c (length c) <= (norm_length - norm_length) * pow2 53
+	/\ eval h1 c (2*norm_length-1) = eval h1 a (norm_length) * eval h1 b (norm_length - norm_length) ))
+let multiplication_lemma_1 h0 h1 c a b =
+  helper_lemma_13 h0 h1 a;
+  helper_lemma_131 h0 h1 b;
+  helper_lemma_15 h0 h1 c;
+  eval_def h1 b 0;
+  cut(eval h1 b 0 = 0)
+
+(* TODO *)
+//TMP#reset-options "--lax"
+
+val helper_lemma_14: h0:heap -> h1:heap -> h2:heap -> c:bigint -> tmp:bigint{disjoint c tmp} ->
+  Lemma
+    (requires (live h0 c /\ live h2 c /\ ~(contains h0 tmp) /\ modifies_0 h0 h1 /\ live h1 tmp /\ modifies_2 c tmp h1 h2))
+    (ensures ((frameOf tmp = frameOf c /\ modifies_1 c h0 h2)
+	      \/ (frameOf tmp <> frameOf c /\ modifies_bufs (frameOf c) (only c) h0 h2
+		  /\ modifies_bufs (frameOf tmp) TSet.empty h0 h2)))
+let helper_lemma_14 h0 h1 h2 c tmp =
+  if frameOf tmp = frameOf c then begin
+    let rid = frameOf tmp in
+    cut(modifies_bufs rid TSet.empty h0 h1);
+    cut(modifies_bufs rid (only c ++ only tmp) h1 h2);
+    cut(~(contains h0 tmp));
+    cut(modifies_bufs rid (only c) h0 h2)
+  end
+  else ()
+
+val multiplication_lemma_2: h0:heap -> h1:heap -> h2:heap -> c:bigint{length c >= 2*norm_length-1} ->
+  a:bigint{disjoint c a} -> b:bigint{disjoint c b} ->
+  tmp:bigint{disjoint a tmp /\ disjoint b tmp /\ disjoint c tmp} -> Lemma
+     (requires (bound27 h0 a /\ norm h0 b /\ live h0 c /\ null h0 c
+	/\ modifies_0 h0 h1 /\ ~(contains h0 tmp) /\ live h1 tmp
+	/\ bound27 h1 a /\ norm h1 b /\ live h1 c /\ null h1 c
+	/\ maxValue h1 c (length c) <= (norm_length - norm_length) * pow2 53
+	/\ eval h1 c (2*norm_length-1) = eval h1 a (norm_length) * eval h1 b (norm_length - norm_length)
+        /\ bound27 h2 a /\ norm h2 b /\ live h2 c
+        /\ modifies_2 c tmp h1 h2
+        /\ eval h2 c (2*norm_length-1) = eval h1 a (norm_length) * eval h1 b (norm_length)
+        /\ maxValue h2 c (length c) <= norm_length * pow2 53 ))
+     (ensures (bound27 h0 a /\ norm h0 b /\ live h0 c /\ bound27 h2 a /\ norm h2 b /\ live h2 c
+       (* /\ modifies_1 c h0 h2 *)
+       /\ ((frameOf tmp = frameOf c /\ modifies_1 c h0 h2)
+	      \/ (frameOf tmp <> frameOf c /\ modifies_bufs (frameOf c) (only c) h0 h2
+		  /\ modifies_bufs (frameOf tmp) TSet.empty h0 h2))
+       /\ eval h2 c (2*norm_length-1) = eval h0 a (norm_length) * eval h0 b (norm_length)
+       /\ maxValue h2 c (length c) <= norm_length * pow2 53 ))
+let multiplication_lemma_2 h0 h1 h2 c a b tmp =
+  helper_lemma_14 h0 h1 h2 c tmp;
+  helper_lemma_13 h0 h1 a;
+  helper_lemma_13 h0 h1 b
+
+
+//TMP#reset-options "--initial_fuel 0 --max_fuel 0"
+
+(* TODO: move a generalized version to buffer *)
+let eq_lemma_fresh h0 h1 a : Lemma
+  (requires (live h0 a /\ fresh_frame h0 h1))
+  (ensures  (live h0 a /\ live h1 a /\ (forall (i:nat). {:pattern (get h1 a i)} i < length a
+			    ==> get h1 a i == get h0 a i)))
+  = ()
+
+//TMP#reset-options "--initial_fuel 0 --max_fuel 0 --z3timeout 10"
+
+(* (\* Code : core multiplication function *\) *)
+(* val multiplication: c:bigint{length c >= 2*norm_length-1} -> a:bigint{disjoint c a} -> *)
+(*   b:bigint{disjoint c b} -> STL unit *)
+(*      (requires (fun h -> live h a /\ live h b /\ live h c *)
+(*        (\* bound27 h a /\ norm h b /\ live h c /\ null h c *\) *)
+(*      )) *)
+(*      (ensures (fun h0 u h1 -> live h1 c /\ modifies_1 c h0 h1 *)
+(*        (\* /\ bound27 h0 a /\ norm h0 b /\ live h0 c /\ bound27 h1 a /\ norm h1 b *\) *)
+(*        (\* /\ eval h1 c (2*norm_length-1) = eval h0 a (norm_length) * eval h0 b (norm_length) *\) *)
+(*        (\* /\ maxValue h1 c (length c) <= norm_length * pow2 53 *\) *)
+(*      )) *)
+(* let multiplication c a b = *)
+(*   let h_init = HST.get() in *)
+(*   push_frame (); *)
+(*   let h0 = HST.get() in *)
+(*   let tmp = create (uint64_to_sint64 0UL) nlength in *)
+(*   let h1 = HST.get() in *)
+(*   multiplication_aux a b nlength c tmp; *)
+(*   let h2 = HST.get() in *)
+(*   lemma_modifies_0_2' c tmp h0 h1 h2; *)
+(*   assert(modifies_2_1 c h0 h2); *)
+(*   pop_frame (); *)
+(*   let hfin = HST.get() in *)
+(*   () *)
+
+
+(*** Modulo ***)
+
+//TMP#reset-options "--initial_fuel 0 --max_fuel 0"
+
+assume val prime_modulo_lemma: unit -> Lemma (pow2 130 % (reveal prime) = 5)
+
+val modulo_lemma: a:nat -> b:pos -> Lemma (requires (a < b)) (ensures (a % b = a))
+  [SMTPat (a % b)]
+let modulo_lemma a b = ()
+
+let satisfiesModuloConstraints (h:heap) (b:bigint) : GTot Type0 =
+  live h b /\ length b >= 2*norm_length-1 && maxValue h b (2*norm_length-1) * 6 < pow2 62
+
+(* TODO *)
+//TMP#reset-options "--lax"
+
+(* val times_5: x:s64{5 * v x < pow2 64} -> Tot (y:s64{v y = 5 * v x}) *)
+(* let times_5 x = *)
+(*   let z = x <<^ 2ul in *)
+(*   x +^ z *)
+
+//TMP#reset-options "--initial_fuel 0 --max_fuel 0"
+
+let reducible (h:heap) (b:bigint) (ctr:nat{ctr < norm_length-1}) : GTot Type0 =
+  live h b /\ length b >= 2*norm_length-1
+  /\ (forall (i:nat). {:pattern (get h b (i+norm_length))}
+      i <= ctr ==> v (get h b i) + 5 * v (get h b (i+norm_length)) < pow2 64)
+
+let times5 (h0:heap) (h1:heap) (b:bigint) (ctr:nat{ctr < norm_length - 1}) : GTot Type0 =
+  live h0 b /\ live h1 b /\ length b >= 2*norm_length-1
+  /\ (forall (i:nat). {:pattern (get h1 b i)}
+       i <= ctr ==> v (get h1 b i) = v (get h0 b i) + 5 * (v (get h0 b (i+norm_length))))
+
+let untouched (h0:heap) (h1:heap) (b:bigint) (ctr:nat) : GTot Type0 =
+  live h0 b /\ live h1 b /\ length b >= 2*norm_length-1
+  /\ (forall (i:nat). {:pattern (get h1 b i)} (i > ctr /\ i < 2*norm_length-1) ==>
+      get h0 b i == get h1 b i)
+
+(* TODO *)
+//TMP#reset-options "--lax"
+
+val pow2_bitweight_lemma_1: ctr:pos -> Lemma (requires (True))
+    (ensures (pow2 (bitweight templ (ctr+norm_length-1)) = pow2 (bitweight templ (ctr-1)) * pow2 (bitweight templ norm_length)))
+let rec pow2_bitweight_lemma_1 ctr =
+  match ctr with
+  | 1 -> ()
+  | _ ->
+    cut(ctr-1+norm_length = ctr+norm_length-1 /\ ctr+norm_length-1 = (ctr-1) + norm_length
+	/\ (ctr+norm_length-1)-1=ctr+norm_length-2);
+    pow2_bitweight_lemma_1 (ctr-1);
+    cut (pow2 (bitweight templ (ctr+norm_length-2)) = pow2 (bitweight templ (ctr-2)) * pow2 (bitweight templ norm_length));
+    cut (bitweight templ (ctr+norm_length-1) = bitweight templ (ctr+norm_length-2) + 26);
+    Math.Lib.pow2_exp_lemma (bitweight templ (ctr+norm_length-2)) 26;
+    cut(pow2 (bitweight templ (ctr+norm_length-1)) = pow2 26 * pow2 (bitweight templ (ctr+norm_length-2)));
+    cut(pow2 (bitweight templ (ctr+norm_length-1)) = pow2 26 * (pow2 (bitweight templ (ctr-2)) * pow2 (bitweight templ norm_length)));
+    paren_mul_right (pow2 26) (pow2 (bitweight templ (ctr-2))) (pow2 (bitweight templ norm_length));
+    cut (pow2 (bitweight templ (ctr+norm_length-1)) = pow2 26 * pow2 (bitweight templ (ctr-2)) * pow2 (bitweight templ norm_length));
+    Math.Lib.pow2_exp_lemma 26 (bitweight templ (ctr-2));
+    cut (pow2 (bitweight templ (ctr+norm_length-1)) = pow2 (26 + bitweight templ (ctr-2)) * pow2 (bitweight templ norm_length))
+
+//TMP#reset-options "--initial_fuel 6 --max_fuel 6"
+
+val bitweight_norm_length_lemma: unit -> Lemma
+  (requires (True))
+  (ensures (bitweight templ norm_length = 130))
+  [SMTPat (bitweight templ norm_length)]
+let bitweight_norm_length_lemma () =
+  ()
+
+
+//TMP#reset-options "--initial_fuel 0 --max_fuel 0"
+
+(* WIP *)
+
+(* TODO: express in terms of general % property *)
+assume val helper_lemma_5: a:nat -> b:nat -> c:nat -> p:pos -> Lemma (ensures ( (a*b+c) % p = ((a % p) * b + c)%p))
+
+val lemma_aux_0: a:int -> b:int -> c:int -> d:int -> Lemma (a * b + c - (a * (b + 5 * d) + c) = - 5 * a * d)
+let lemma_aux_0 a b c d = ()
+
+//TMP#reset-options "--z3timeout 100"
+#set-options "--lax" // TODO
+
+val freduce_degree_lemma_2: h0:heap -> h1:heap -> b:bigint{live h1 b /\ live h0 b /\ length b >= 2 * norm_length - 1} -> ctr:pos{ctr < norm_length-1} -> Lemma
+    (requires ((forall (i:nat). {:pattern (v (get h1 b i))}
+	(i < length b /\ i <> ctr) ==> v (get h1 b i) = v (get h0 b i)) 
+	/\ v (get h1 b ctr) = v (get h0 b ctr) + 5 * v (get h0 b (ctr+norm_length)) ))
+    (ensures (eval h0 b (norm_length+1+ctr) % (reveal prime) = eval h1 b (norm_length+ctr) % (reveal prime)))
+let freduce_degree_lemma_2 h0 h1 b ctr =
+  let prime = reveal prime in 
+  cut (ctr+norm_length = norm_length+ctr /\ (norm_length+1+ctr)-1 = norm_length + ctr /\ norm_length+ctr = (ctr+1)+norm_length-1); 
+  cut (eval h0 b (norm_length+1+ctr) = pow2 (bitweight templ (norm_length+ctr)) * v (get h0 b (norm_length+ctr)) + eval h0 b (ctr+norm_length)); 
+  pow2_bitweight_lemma_1 (ctr+1); 
+  cut(pow2 (bitweight templ (norm_length+ctr)) = pow2 130 * pow2 (bitweight templ ctr)); 
+  paren_mul_left (pow2 130) (pow2 (bitweight templ ctr)) (v (get h0 b (norm_length+ctr))); 
+  paren_mul_right (pow2 130) (pow2 (bitweight templ ctr)) (v (get h0 b (norm_length+ctr))); 
+  cut (eval h0 b (norm_length+1+ctr) = (pow2 130 * pow2 (bitweight templ ctr)) * v (get h0 b (norm_length+ctr)) + eval h0 b (norm_length+ctr)); 
+  helper_lemma_5 (pow2 130) (pow2 (bitweight templ ctr) * v (get h0 b (norm_length+ctr))) (eval h0 b (norm_length+ctr)) prime; 
+  cut (eval h0 b (norm_length+1+ctr) % prime = ((pow2 130 % prime) * pow2 (bitweight templ ctr) * v (get h0 b (norm_length+ctr)) + eval h0 b (norm_length+ctr)) % prime); 
+  prime_modulo_lemma (); 
+  cut (eval h0 b (norm_length+1+ctr) % prime = (5 * pow2 (bitweight templ ctr) * v (get h0 b (norm_length+ctr)) + eval h0 b (norm_length+ctr)) % prime); 
+  eval_eq_lemma h0 h1 b b ctr; 
+  cut (eval h0 b (ctr+1) = pow2 (bitweight templ ctr) * v (get h0 b ctr) + eval h0 b ctr); 
+  cut (eval h1 b (ctr+1) = pow2 (bitweight templ ctr) * (v (get h0 b ctr) + 5 * v (get h0 b (norm_length+ctr))) + eval h0 b ctr); 
+  lemma_aux_0 (pow2 (bitweight templ ctr)) (v (get h0 b ctr)) (eval h0 b ctr) (v (get h0 b (norm_length+ctr)));
+  cut (eval h0 b (ctr+1) - eval h1 b (ctr+1) = - 5 * pow2 (bitweight templ ctr) * v (get h0 b (norm_length+ctr)) /\ True); 
+  distributivity_add_right (pow2 (bitweight templ ctr)) (v (get h0 b ctr)) (5 * v (get h0 b (norm_length+ctr))); 
+  eval_partial_eq_lemma h0 h1 b b (ctr+1) (norm_length+ctr); 
+  cut (eval h0 b (norm_length+ctr) - eval h0 b (ctr+1) = eval h1 b (norm_length+ctr) - eval h1 b (ctr+1) /\ True); 
+  cut ( eval h0 b (norm_length+1+ctr) % prime = (5 * pow2 (bitweight templ ctr) * v (get h0 b (norm_length+ctr)) + eval h1 b (norm_length+ctr) + eval h0 b (ctr+1) - eval h1 b (ctr+1)) % prime /\ True); 
+  cut ( eval h0 b (norm_length+1+ctr) % prime = (5 * pow2 (bitweight templ ctr) * v (get h0 b (norm_length+ctr)) + eval h1 b (norm_length+ctr) - 5 * pow2 (bitweight templ ctr) * v (get h0 b (norm_length+ctr))) % prime /\ True); 
+  cut ( eval h0 b (norm_length+1+ctr) % prime = (eval h1 b (norm_length+ctr) ) % prime /\ True)
+
+//TMP#reset-options "--z3timeout 50"
+#set-options "--lax" // OK
+
+val freduce_degree_lemma:
+  h0:heap -> h1:heap -> b:bigint{live h1 b /\ live h0 b /\ length b >= 2 * norm_length - 1} -> 
+  ctr:nat{ctr < norm_length-1} -> Lemma
+    (requires ((forall (i:nat). {:pattern (v (get h1 b i))}
+	(i < length b /\ i <> ctr) ==> v (get h1 b i) = v (get h0 b i)) 
+      /\ v (get h1 b ctr) = v (get h0 b ctr) + 5 * v (get h0 b (ctr+norm_length)) ))
+    (ensures (eval h0 b (norm_length+1+ctr) % (reveal prime) = eval h1 b (norm_length+ctr) % (reveal prime)))  
+let freduce_degree_lemma h0 h1 b ctr =
+  let prime = reveal prime in
+  if ctr = 0 then (
+    helper_lemma_5 (pow2 130) (v (get h0 b norm_length)) (eval h0 b norm_length) prime;
+    prime_modulo_lemma ();
+    cut(eval h0 b 1 = v (get h0 b 0) /\ eval h1 b 1 = v (get h0 b 0) + 5 * v (get h0 b norm_length)); 
+    eval_partial_eq_lemma h0 h1 b b 1 norm_length;
+    cut(eval h1 b norm_length - eval h1 b 1 = eval h0 b norm_length - eval h0 b 1)
+  ) else (
+    freduce_degree_lemma_2 h0 h1 b ctr
+  )
+
+//TMP#reset-options "--z3timeout 100"
+#set-options "--lax" // TODO
+
+(* val freduce_degree':  *)
+(*   b:bigint -> ctr:u32{w ctr < norm_length - 1} -> STL unit  *)
+(*     (requires (fun h -> reducible h b (w ctr)))  *)
+(*     (ensures (fun h0 _ h1 -> untouched h0 h1 b (w ctr) /\ times5 h0 h1 b (w ctr) *)
+(*       /\ eval h1 b (norm_length) % reveal prime = eval h0 b (norm_length+1+w ctr) % reveal prime *)
+(*       /\ modifies_1 b h0 h1)) *)
+(* let rec freduce_degree' b ctr' = *)
+(*   let h0 = HST.get() in *)
+(*   if U32.eq ctr' 0ul then begin *)
+(*     let b5ctr = index b (0ul+|nlength) in  *)
+(*     let bctr = index b 0ul in *)
+(*     let b5ctr = times_5 b5ctr in *)
+(*     let bctr = bctr +^ b5ctr in  *)
+(*     upd b 0ul bctr; *)
+(*     let h1 = HST.get() in *)
+(*     freduce_degree_lemma h0 h1 b 0; *)
+(*     cut (eval h0 b (norm_length+1+0) % reveal prime = eval h1 b (norm_length+0) % reveal prime); *)
+(*     cut (eval h0 b (norm_length+1) % reveal prime = eval h1 b (norm_length+0) % reveal prime) *)
+(*     end *)
+(*   else begin *)
+(*     let ctr = ctr' in *)
+(*     let b5ctr = index b (ctr +| nlength) in  *)
+(*     let bctr = index b ctr in *)
+(*     let b5ctr = times_5 b5ctr in *)
+(*     let bctr = bctr +^ b5ctr in  *)
+(*     upd b ctr bctr; *)
+(*     let h1 = HST.get() in *)
+(*     freduce_degree_lemma h0 h1 b (w ctr);  *)
+(*     cut (eval h0 b (norm_length+1+w ctr) % reveal prime = eval h1 b (norm_length+w ctr) % reveal prime); *)
+(*     cut(reducible h1 b (w ctr-1));  *)
+(*     freduce_degree' b (ctr-|1ul);  *)
+(*     let h2 = HST.get() in  *)
+(*     cut (forall (i:nat). {:pattern (v (get h1 b i))} (i > w ctr /\ i < 2*norm_length-1) ==> *)
+(* 	   v (get h1 b i) = v (get h0 b i));  *)
+(*     cut(untouched h0 h2 b (w ctr)); *)
+(*     cut (times5 h0 h2 b (w ctr)) ; *)
+(*     () *)
+(*   end *)
+
+//TMP#reset-options
+
+val aux_lemma_4': h:heap -> b:bigint -> Lemma
+  (requires (satisfiesModuloConstraints h b))
+  (ensures (reducible h b (norm_length-2)))
+let aux_lemma_4' h b =
+  maxValue_lemma_aux h b (2*norm_length-1);
+  Math.Lib.pow2_increases_lemma 64 62;
+  ()
+  
+val aux_lemma_5': h0:heap -> h1:heap -> b:bigint -> Lemma
+  (requires (live h0 b /\ satisfiesModuloConstraints h0 b /\ times5 h0 h1 b (norm_length-2)
+      /\ untouched h0 h1 b (norm_length-2)))
+  (ensures (live h0 b /\ satisfiesModuloConstraints h0 b /\ times5 h0 h1 b (norm_length-2)
+    /\ (forall (i:nat). i <= norm_length ==> v (get h1 b i) < pow2 62)))
+let aux_lemma_5' h0 h1 b = 
+  maxValue_lemma_aux h0 b (2*norm_length-1)
+
+(* val freduce_degree: b:bigint -> STL unit  *)
+(*   (requires (fun h -> live h b /\ satisfiesModuloConstraints h b))  *)
+(*   (ensures (fun h0 _ h1 -> live h0 b /\ live h1 b /\ satisfiesModuloConstraints h0 b *)
+(*     /\ modifies_1 b h0 h1 *)
+(*     /\ (forall (i:nat). {:pattern (v (get h1 b i))} i <= norm_length ==>  *)
+(* 	v (get h1 b i) < pow2 62) *)
+(*     /\ eval h1 b norm_length % reveal prime = eval h0 b (2*norm_length-1) % reveal prime)) *)
+(* let freduce_degree b =  *)
+(*   let h0 = HST.get() in *)
+(*   aux_lemma_4' h0 b;  *)
+(*   freduce_degree' b (nlength-|2ul);  *)
+(*   let h1 = HST.get() in *)
+(*   aux_lemma_5' h0 h1 b *)
+
+val pow2_bitweight_lemma: ctr:nat -> Lemma 
+    (requires (True)) 
+    (ensures (pow2 (bitweight templ (ctr+1)) = pow2 (bitweight templ ctr) * pow2 (templ ctr)))
+let pow2_bitweight_lemma ctr =
+  Math.Lib.pow2_exp_lemma (bitweight templ ctr) (templ ctr);
+  ()
+
+val helper_lemma_2: pb:nat -> pc:pos -> a0:nat -> b:nat ->
+  Lemma  (ensures ((pb*pc) * a0/pc + (pb * (a0 % pc) + b) = pb * a0 + b))
+let helper_lemma_2 pb pc a0 b = ()
+
+//TMP#reset-options "--z3timeout 100"
+#set-options "--lax" // TODO
+
+val eval_carry_lemma: ha:heap -> a:bigint{live ha a /\ length a >= norm_length+1} -> 
+  hb:heap -> b:bigint{live hb b /\ length b >= norm_length+1} -> ctr:nat{ctr < norm_length} -> Lemma
+    (requires (v (get hb b ctr) = v (get ha a ctr) % pow2 (templ ctr)
+      /\ v (get hb b (ctr+1)) = v (get ha a (ctr+1)) + v (get ha a ctr) / pow2 (templ ctr)
+      /\ (forall (i:nat). {:pattern (v (get hb b i))}
+	  (i < norm_length+1 /\ i <> ctr /\ i <> ctr+1) ==> v (get hb b i) = v (get ha a i)) ))
+    (ensures (eval hb b (norm_length+1) = eval ha a (norm_length+1)))
+let eval_carry_lemma ha a hb b ctr =
+  eval_eq_lemma ha hb a b ctr;
+  cut(eval hb b (ctr+2) = pow2 (bitweight templ (ctr+1)) * v (get hb b (ctr+1)) + eval hb b (ctr+1)); 
+  cut(eval hb b (ctr+2) = pow2 (bitweight templ (ctr+1)) * v (get hb b (ctr+1)) + (pow2 (bitweight templ ctr) * v (get hb b ctr) + eval hb b ctr));  
+  cut(eval hb b (ctr+2) = pow2 (bitweight templ (ctr+1)) * (v (get ha a (ctr+1)) + v (get ha a ctr) / pow2 (templ ctr)) + (pow2 (bitweight templ ctr) * (v (get ha a ctr) % pow2 (templ ctr)) + eval hb b ctr)); 
+  distributivity_add_right (pow2 (bitweight templ (ctr+1))) (v (get ha a (ctr+1))) (v (get ha a ctr) / pow2 (templ ctr));
+  cut(eval hb b (ctr+2) = 
+	      pow2 (bitweight templ (ctr+1)) * v (get ha a (ctr+1))
+	      + pow2 (bitweight templ (ctr+1)) * v (get ha a ctr) / pow2 (templ ctr) 
+	      + (pow2 (bitweight templ ctr) * (v (get ha a ctr) % pow2 (templ ctr)) + eval hb b ctr));
+  pow2_bitweight_lemma ctr; 
+  cut(eval hb b (ctr+2) = 
+	      pow2 (bitweight templ (ctr+1)) * v (get ha a (ctr+1)) 
+	      + (pow2 (bitweight templ ctr) * pow2 (templ ctr)) * v (get ha a ctr) / pow2 (templ ctr) 
+	      + (pow2 (bitweight templ ctr) * (v (get ha a ctr) % pow2 (templ ctr)) + eval hb b ctr));
+  helper_lemma_2 (pow2 (bitweight templ ctr)) (pow2 (templ ctr)) (v (get ha a ctr)) (eval hb b ctr); 
+  cut( eval hb b (ctr+2) = 
+	      pow2 (bitweight templ (ctr+1)) * v (get ha a (ctr+1)) 
+	      + (pow2 (bitweight templ ctr) * v (get ha a ctr) + eval hb b ctr));  
+  cut(eval hb b (ctr+2) = eval ha a (ctr+2)); 
+  eval_partial_eq_lemma ha hb a b (ctr+2) (norm_length+1)
+
+//TMP#reset-options
+
+val helper_lemma_4: a:nat -> b:nat -> c:pos -> size:pos{size > c} ->
+  Lemma (requires (a < pow2 (size-1) /\ b < pow2 (size-c)))
+	(ensures (a + b < pow2 size))
+let helper_lemma_4 a b c size = 
+  if size-1 > size - c then begin
+    Math.Lib.pow2_increases_lemma (size-1) (size-c) ;
+    ()
+    end
+  else ()
+
+val auxiliary_lemma_1': bip1:s64 -> c:s64 -> Lemma
+    (requires (v bip1 < pow2 62 /\ v c < pow2 (64 - 26)))
+    (ensures (v bip1 + v c < pow2 64)) 
+let auxiliary_lemma_1' bip1 c =
+  helper_lemma_4 (v bip1) (v c) 26 64
+
+val auxiliary_lemma_2: bip1:s64 -> c:s64 -> Lemma
+    (requires (v bip1 < pow2 26 /\ v c < pow2 15))
+    (ensures (v bip1 + v c < pow2 27)) 
+let auxiliary_lemma_2 bip1 c =
+  helper_lemma_4 (v bip1) (v c) 12 27
+
+(* TODO: move somewhere more appropriate *)
+assume MaxUint32: FStar.UInt.max_int 32 = 4294967295
+
+val mod2_26: a:s64 -> Tot (b:s64{v b = v a % pow2 26})
+let mod2_26 a = 
+  admit(); // TODO
+  let mask = shift_left (uint64_to_sint64 1UL) 26ul in
+  Math.Lib.pow2_increases_lemma 64 26;
+  let mask = mask -^ (uint64_to_sint64 1UL) in
+  let res = a &^ mask in
+  (* SInt.ulogand_lemma_4 #64 a 26 mask; *)
+  res
+
+let carriable (h:heap) (b:bigint) (ctr:nat{ctr <= norm_length}) : GTot Type0 =
+  live h b /\ length b >= norm_length + 1  
+  /\ (forall (i:nat). {:pattern (v (get h b i))}
+      (i > ctr /\ i <= norm_length) ==> v (get h b i) < pow2 62)
+
+let carried (h1:heap) (b:bigint) (ctr:nat{ctr <= norm_length}) : GTot Type0 =
+  live h1 b /\ length b >= norm_length + 1
+  /\ (forall (i:nat). {:pattern (v (get h1 b i))} i < ctr ==> v (get h1 b i) < pow2 (templ ctr))
+  /\ (ctr <> norm_length ==> v (get h1 b norm_length) = 0)
+  /\ (ctr = norm_length ==> v (get h1 b norm_length) < pow2 37)
+  
+let carried' (h1:heap) (b:bigint) (ctr:nat{ctr <= norm_length}) : GTot Type0 =
+  live h1 b /\ length b >= norm_length + 1
+  /\ (forall (i:nat). {:pattern (v (get h1 b i))} (i >= ctr /\ i < norm_length) ==> v (get h1 b i) < pow2 (templ ctr))
+  /\ v (get h1 b norm_length) < pow2 37
+  
+let untouched_2 (h0:heap) (h1:heap) (b:bigint) (ctr:nat) : GTot Type0 =
+  live h0 b /\ live h1 b /\ length b >= norm_length+1 
+  /\ (forall (i:nat). {:pattern (get h1 b i)}
+      ((i < ctr \/ i >= norm_length+1) /\ i < length b) ==> v (get h0 b i) = v (get h1 b i))
+
+//TMP#reset-options "--z3timeout 100"
+#set-options "--lax" // TODO
+
+(* val carry: b:bigint -> ctr:u32{U32.v ctr <= norm_length} -> ST unit *)
+(*     (requires (fun h -> carriable h b (U32.v ctr) /\ carried h b (U32.v ctr))) *)
+(*     (ensures (fun h0 _ h1 -> carried h1 b norm_length /\ untouched_2 h0 h1 b (U32.v ctr) *)
+(*       /\ eval h1 b (norm_length+1) = eval h0 b (norm_length+1) *)
+(*       /\ modifies_1 b h0 h1 )) *)
+(* let rec carry b i = *)
+(*   let h0 = HST.get() in *)
+(*   if U32.eq i nlength then admit() *)
+(*   else begin  *)
+(*     let bi = index b i in *)
+(*     let ri = mod2_26 bi in *)
+(*     upd b i ri; *)
+(*     let h1 = HST.get() in *)
+(*     let c = (bi >>^ 26ul) in *)
+(*     cut (v c = (v bi) / (pow2 26)); *)
+(*     Math.Lib.pow2_div_lemma 64 26; *)
+(*     (\* TODO *\) *)
+(*     assume (v c < pow2 (64 - 26)); *)
+(*     assert(live h1 b); *)
+(*     assert(U32.v i + 1 < length b);  *)
+(*     let bip1 = index b (i+|1ul) in *)
+(*     auxiliary_lemma_1' bip1 c;  *)
+(*     let z = bip1 +^ c in *)
+(*     upd b (i+|1ul) z; *)
+(*     let h2 = HST.get() in *)
+(*     eval_carry_lemma h0 b h2 b (U32.v i); *)
+(*     carry b (i+|1ul) *)
+(*   end  *)
+
+//TMP#reset-options "--z3timeout 20"
+#set-options "--lax" // OK
+
+(* val carry_top_to_0: b:bigint -> STL unit *)
+(*     (requires (fun h -> carried h b norm_length /\ length b >= 2*norm_length-1 *)
+(*       /\ v (get h b 0) + 5 * v (get h b norm_length) < pow2 63)) *)
+(*     (ensures (fun h0 _ h1 -> carried h0 b norm_length /\ carried' h1 b 1 *)
+(*       /\ eval h1 b norm_length % (reveal prime) = eval h0 b (norm_length+1) % (reveal prime) *)
+(*       /\ v (get h1 b 0) = v (get h0 b 0) + 5 * v (get h0 b norm_length) *)
+(*       /\ (forall (i:nat). {:pattern (v (get h1 b i))} (i > 0 /\ i < length b) ==>  *)
+(* 	  v (get h1 b i) = v (get h0 b i)) *)
+(*       /\ modifies_1 b h0 h1))       *)
+(* let carry_top_to_0 b = *)
+(*   Math.Lib.pow2_increases_lemma 64 63; *)
+(*   let h0 = HST.get() in *)
+(*   let b0 = index b 0ul in *)
+(*   let btop = index b nlength in  *)
+(*   let btop_5 = times_5 btop in *)
+(*   upd b 0ul (b0 +^ btop_5); *)
+(*   let h1 = HST.get() in *)
+(*   freduce_degree_lemma h0 h1 b 0 *)
+
+//TMP#reset-options
+
+let carriable2 (h:heap) (b:bigint) (ctr:pos{ctr<=norm_length}) : GTot Type0 =
+  live h b /\ length b >= norm_length + 1
+  /\ (forall (i:nat). {:pattern (v (get h b i))} i < ctr ==> v (get h b i) < pow2 26)
+  /\ (forall (i:nat). {:pattern (v (get h b i))} (i > ctr /\ i < norm_length) ==> v (get h b i) < pow2 26)
+  /\ (ctr < norm_length ==> v (get h b norm_length) = 0)
+  /\ (ctr = norm_length ==> v (get h b norm_length) < 2)
+  /\ v (get h b ctr) < pow2 26 + pow2 15
+  /\ (v (get h b ctr) >= pow2 26 ==> (
+      forall (i:nat). {:pattern (v (get h b i))} ( i < ctr /\ i > 0) ==> v (get h b i) < pow2 15))
+  /\ ((ctr = norm_length /\ v (get h b norm_length) = 1) ==> 
+      (forall (i:nat). {:pattern (v (get h b i))} (i > 0 /\ i < norm_length) ==> v (get h b i) < pow2 15))
+
+val lemma_aux: a:nat -> b:pos -> Lemma (Math.Lib.div a b > 0 ==> a >= b)
+let lemma_aux a b = 
+  ()
+
+(* TODO: express in terms of % properties *)
+assume val lemma_aux_2: a:s64 -> Lemma ((v a < pow2 26+pow2 15 /\ v a >= pow2 26) ==> v a % pow2 26 < pow2 15)
+
+//TMP#reset-options "--z3timeout 100"
+#set-options "--lax" // OK
+
+(* val carry2_aux: b:bigint -> ctr:u32{w ctr > 0 /\ w ctr <= norm_length} -> STL unit *)
+(*   (requires (fun h -> carriable2 h b (w ctr))) *)
+(*   (ensures (fun h0 _ h1 -> carriable2 h0 b (w ctr) /\ carriable2 h1 b norm_length *)
+(*     /\ eval h1 b (norm_length+1) = eval h0 b (norm_length+1) *)
+(*     /\ modifies_1 b h0 h1 )) *)
+(* let rec carry2_aux b i =  *)
+(*   let h0 = HST.get() in *)
+(*   if U32.eq i nlength then () *)
+(*   else begin *)
+(*     let bi = index b i in  *)
+(*     let ri = mod2_26 bi in *)
+(*     lemma_aux_2 bi; *)
+(*     cut (v ri < pow2 (templ (w i)));  *)
+(*     upd b i ri;  *)
+(*     let h1 = HST.get() in *)
+(*     let c = (bi >>^ 26ul) in *)
+(*     // In the spec of >>, TODO *)
+(*     assume(v c < 2);  *)
+(*     let bip1 = index b (i+|1ul) in *)
+(*     auxiliary_lemma_2 bip1 c;  *)
+(*     Math.Lib.pow2_increases_lemma 64 27; *)
+(*     Math.Lemmas.pow2_double_sum 26; *)
+(*     Math.Lib.pow2_increases_lemma 26 15; *)
+(*     let z = bip1 +^ c in  *)
+(*     cut (v z = v bip1 + v c /\ v c < 2 /\ v bip1 < pow2 26);  *)
+(*     cut (v z >= pow2 26 ==> v c = 1);  *)
+(*     cut (v c > 0 ==> v (get h0 b (w i)) / (pow2 26) > 0 ==> v (get h0 b (w i)) >= pow2 26); *)
+(*     cut (v z >= pow2 26 ==> v (get h1 b (w i)) < pow2 15);  *)
+(*     upd b (i+|1ul) z; *)
+(*     let h2 = HST.get() in  *)
+(*     cut (v z >= pow2 26 ==> v c = 1);  *)
+(*     eval_carry_lemma h0 b h2 b (w i);  *)
+(*     carry2_aux b (i+|1ul) *)
+(*   end *)
+
+//TMP#reset-options
+
+val pow2_3_lemma: unit -> Lemma (pow2 3 = 8)
+let pow2_3_lemma () = 
+  ()
+
+//TMP#reset-options "--z3timeout 100"
+#set-options "--lax" // TODO
+
+(* val carry2: b:bigint -> STL unit *)
+(*   (requires (fun h -> carried h b norm_length /\ length b >= 2*norm_length-1)) *)
+(*   (ensures (fun h0 _ h1 -> carried h0 b norm_length /\ carriable2 h1 b norm_length  *)
+(*     /\ eval h1 b (norm_length+1) % reveal prime = eval h0 b (norm_length+1) % reveal prime *)
+(*     /\ modifies_1 b h0 h1)) *)
+(* let rec carry2 b =  *)
+(*   let h0 = HST.get() in *)
+(*   pow2_3_lemma (); *)
+(*   Math.Lib.pow2_exp_lemma 3 37; *)
+(*   Math.Lib.pow2_increases_lemma 40 37; *)
+(*   Math.Lib.pow2_increases_lemma 40 26; *)
+(*   Math.Lemmas.pow2_double_sum 40; *)
+(*   Math.Lib.pow2_increases_lemma 63 41; *)
+(*   carry_top_to_0 b; *)
+(*   let h1 = HST.get() in *)
+(*   upd b nlength (uint64_to_sint64 0UL); *)
+(*   let h2 = HST.get() in *)
+(*   eval_eq_lemma h1 h2 b b norm_length; *)
+(*   cut ( eval h2 b (norm_length+1) = eval h1 b (norm_length));  *)
+(*   let bi = index b 0ul in  *)
+(*   let ri = mod2_26 bi in *)
+(*   cut (v ri < pow2 26);  *)
+(*   upd b 0ul ri;  *)
+(*   let h3 = HST.get() in *)
+(*   let c = (bi >>^ 26ul) in *)
+(*   cut (v bi < pow2 41);  *)
+(*   // In the spec of >>, TODO *)
+(*   assume (v c < pow2 15);  *)
+(*   let bip1 = index b 1ul in  *)
+(*   auxiliary_lemma_2 bip1 c;  *)
+(*   Math.Lib.pow2_increases_lemma 64 27; *)
+(*   Math.Lemmas.pow2_double_sum 26; *)
+(*   Math.Lib.pow2_increases_lemma 26 15; *)
+(*   let z = bip1 +^ c in  *)
+(*   upd b 1ul z; *)
+(*   let h4 = HST.get() in  *)
+(*   eval_carry_lemma h2 b h4 b 0;  *)
+(*   cut(carriable2 h4 b 1); *)
+(*   carry2_aux b 1ul *)
+
+//TMP#reset-options "--z3timeout 100"
+
+(* val last_carry: b:bigint -> STL unit *)
+(*   (requires (fun h -> carriable2 h b norm_length /\ length b >= 2*norm_length-1)) *)
+(*   (ensures (fun h0 _ h1 -> carriable2 h0 b norm_length /\ norm h1 b *)
+(*     /\ eval h1 b norm_length % reveal prime = eval h0 b (norm_length+1) % reveal prime *)
+(*     /\ modifies_1 b h0 h1)) *)
+(* let last_carry b = *)
+(*   let h0 = HST.get() in *)
+(*   let b0 = index b 0ul in *)
+(*   let btop = index b nlength in  *)
+(*   cut (v b0 < pow2 26 /\ v btop < 2);  *)
+(*   pow2_3_lemma (); *)
+(*   cut (5 * v btop < pow2 3 /\ True);  *)
+(*   Math.Lib.pow2_increases_lemma 26 3; *)
+(*   Math.Lemmas.pow2_double_sum 26; *)
+(*   Math.Lib.pow2_increases_lemma 64 27; *)
+(*   cut(v b0 + 5 * v btop < pow2 27 /\ True);  *)
+(*   let btop_5 = times_5 btop in   *)
+(*   upd b 0ul (b0 +^ btop_5);  *)
+(*   let h1 = HST.get() in *)
+(*   freduce_degree_lemma h0 h1 b 0; *)
+(*   upd b nlength (uint64_to_sint64 0UL); *)
+(*   let h2 = HST.get() in *)
+(*   eval_eq_lemma h1 h2 b b norm_length; *)
+(*   cut (eval h2 b (norm_length+1) = eval h1 b norm_length); *)
+(*   let bi = index b 0ul in  *)
+(*   let ri = mod2_26 bi in *)
+(* //  assert(v ri < pow2 26);  *)
+(*   upd b 0ul ri;  *)
+(*   let h3 = HST.get() in *)
+(*   let c = (bi >>^ 26ul) in *)
+(*   cut (v bi < pow2 26 + 5); *)
+(*   cut (v bi >= pow2 26 ==> v (get h3 b 1) < pow2 15); *)
+(*   // In the spec of >>, TODO *)
+(*   assume (v bi >= pow2 26 ==> v c = 1); *)
+(*   let bip1 = index b 1ul in *)
+(*   auxiliary_lemma_2 bip1 c; *)
+(*   Math.Lib.pow2_increases_lemma 64 27; *)
+(*   Math.Lemmas.pow2_double_sum 26; *)
+(*   Math.Lib.pow2_increases_lemma 26 15; *)
+(*   let z = bip1 +^ c in *)
+(*   upd b 1ul z; *)
+(*   let h4 = HST.get() in *)
+(*   eval_carry_lemma h2 b h4 b 0; *)
+(*   cut (v (get h4 b 1) < pow2 26); *)
+(*   cut (norm h4 b); *)
+(*   () *)
+
+(* val modulo: b:bigint -> ST unit *)
+(*   (requires (fun h -> live h b /\ satisfiesModuloConstraints h b)) *)
+(*   (ensures (fun h0 _ h1 -> live h0 b /\ satisfiesModuloConstraints h0 b /\ norm h1 b *)
+(*     /\ eval h1 b norm_length % reveal prime = eval h0 b (2*norm_length-1) % reveal prime *)
+(*     /\ modifies_1 b h0 h1)) *)
+(* let modulo b = *)
+(*   let h0 = HST.get() in *)
+(*   freduce_degree b; *)
+(*   let h1 = HST.get() in *)
+(*   upd b nlength (uint64_to_sint64 0UL); *)
+(*   let h2 = HST.get() in *)
+(*   eval_eq_lemma h1 h2 b b norm_length; *)
+(*   cut (eval h2 b (norm_length+1) = eval h1 b norm_length); *)
+(*   carry b 0ul; *)
+(*   let h3 = HST.get() in *)
+(*   carry2 b; *)
+(*   let h4 = HST.get() in *)
+(*   last_carry b *)
+
+(* val freduce_coefficients: b:bigint -> ST unit *)
+(*   (requires (fun h -> live h b   *)
+(*     /\ (forall (i:nat). {:pattern (v (get h b i))} i < norm_length ==> v (get h b i) < pow2 62))) *)
+(*   (ensures (fun h0 _ h1 -> live h0 b /\ norm h1 b  *)
+(*     /\ eval h1 b norm_length % reveal prime = eval h0 b norm_length % reveal prime *)
+(*     /\ modifies_1 b h0 h1)) *)
+(* let freduce_coefficients b =  *)
+(*   let h0 = HST.get() in *)
+(*   let tmp = create (uint64_to_sint64 0UL) (U32.mul 2ul nlength-|1ul) in *)
+(*   let h1 = HST.get() in *)
+(*   eq_lemma_0 h0 h1 b; *)
+(*   eval_eq_lemma h0 h1 b b norm_length; *)
+(*   blit b 0ul tmp 0ul nlength; *)
+(*   let h2 = HST.get() in *)
+(*   eval_eq_lemma h1 h2 b tmp norm_length; *)
+(*   cut (forall (i:nat). {:pattern (v (get h2 tmp i))} i < norm_length ==> v (get h2 tmp i) = v (get h0 b i));  *)
+(*   carry tmp 0ul; *)
+(*   carry2 tmp; *)
+(*   last_carry tmp; *)
+(*   let h = HST.get() in *)
+(*   blit tmp 0ul b 0ul nlength; *)
+(*   let h' = HST.get() in *)
+(*   eval_eq_lemma h h' tmp b norm_length; *)
+(*   cut (forall (i:nat). {:pattern (v (get h tmp i))} i < norm_length ==> v (get h tmp i) < pow2 26);  *)
+(*   cut (forall (i:nat). {:pattern (v (get h' b i))} i < norm_length ==> v (get h' b (0+i)) = v (get h tmp (0+i))) *)
+
+(*** Finalization ***)
+
+#set-options "--lax" // Never done
+
+(* val finalize: b:bigint -> ST unit *)
+(*   (requires (fun h -> norm h b)) *)
+(*   (ensures (fun h0 _ h1 -> norm h0 b /\ norm h1 b *)
+(*     /\ modifies_1 b h0 h1 *)
+(*     /\ eval h1 b norm_length = eval h0 b norm_length % reveal prime)) *)
+(* let finalize b = *)
+(*   let mask_26 = ((uint64_to_sint64 1UL) <<^ 26ul) -^ (uint64_to_sint64 1UL) in *)
+(*   let mask2_26m5 = mask_26 -^ (uint64_to_sint64 1UL <<^ 2ul) in *)
+(*   let b0 = index b 0ul in *)
+(*   let b1 = index b 1ul in *)
+(*   let b2 = index b 2ul in *)
+(*   let b3 = index b 3ul in *)
+(*   let b4 = index b 4ul in *)
+(*   let mask = Hacl.UInt64.eq_mask b4 mask_26 in *)
+(*   let mask = Hacl.UInt64.eq_mask b3 mask_26 &^ mask in *)
+(*   let mask = Hacl.UInt64.eq_mask b2 mask_26 &^ mask in *)
+(*   let mask = Hacl.UInt64.eq_mask b1 mask_26 &^ mask in *)
+(*   let mask = Hacl.UInt64.gte_mask b0 mask2_26m5 &^ mask in *)
+(*   upd b 0ul (b0 -^ (mask &^ mask2_26m5)); *)
+(*   upd b 1ul (b1 -^ (b1 &^ mask)); *)
+(*   upd b 2ul (b2 -^ (b2 &^ mask)); *)
+(*   upd b 3ul (b3 -^ (b3 &^ mask)); *)
+(*   upd b 4ul (b4 -^ (b4 &^ mask)); *)
+(*   () *)
